examples/heapsort/downheap_why.v
@@ -17,7 +17,7 @@ Save.
 
 Implicit Arguments On.
 
-Inductive select_son [N:Z; t:(array N Z); k,n,j:Z] : Prop :=
+Inductive select_son [t:(array Z); k,n,j:Z] : Prop :=
     select_left_son : 
       `j = 2*k+1` -> (`2*k+2 <= n` -> (Zge #t[j] #t[`2*k+2`])) 
         -> (select_son t k n j)
@@ -29,18 +29,18 @@ Implicit Arguments Off.
 
 (* The correctness of downheap requires the two following lemmas *)
 
-Lemma Lemma_1 : (N:Z)(t0,t1,t2:(array N Z))
+Lemma Lemma_1 : (t0,t1,t2:(array Z))
     (n0,k0,j':Z)
     `2*k0+1 <= n0`
  -> (select_son t0 k0 n0 j')
  -> `(access   t0 k0) < (access   t0 j')`
  -> (exchange t1 t0 k0 j')
  -> `0 <= k0 <= n0`
- -> `n0 < N`
+ -> `n0 < (array_length t0)`
  -> ((i:Z)`k0+1 <= i <= n0`->(heap t0 n0 i))
  -> ((i:Z)`j' <= i <= n0`->(heap t2 n0 i))
  -> ((i:Z)
-        `0 <= i < j'`\/`j' < i < 2*j'+1`\/`n0 < i < N`
+        `0 <= i < j'`\/`j' < i < 2*j'+1`\/`n0 < i < (array_length t0)`
         ->`(access   t2 i) = (access   t1 i)`)
  -> ((v:Z)(inftree t1 n0 v j')->(inftree t2 n0 v j'))
  -> (i:Z)`k0 < i < j'`->(heap t2 n0 i).
@@ -49,34 +49,34 @@ Intros. Apply heap_cons.
 Elim H0; Omega'.
 (* branch 2i+1 *)
 Intro. Rewrite (H7 i). Rewrite (H7 `2*i+1`).
-Decompose [exchange] H2. Rewrite (H15 i). Rewrite (H15 `2*i+1`).
-Generalize H10. Elim (H5 i); Intros. Exact (H17 H23).
+Decompose [exchange] H2. Rewrite (H16 i). Rewrite (H16 `2*i+1`).
+Generalize H10. Elim (H5 i); Intros. Exact (H18 H24).
 Omega'. Omega'. Omega'.
 Elim H0; Omega'. Omega'. Omega'. Omega'.
 Elim H0; Omega'. Elim H0; Omega'. 
 Intro. Apply H6; Elim H0; Omega'.
 (* branch 2i+2 *)
 Intro. Rewrite (H7 i). Rewrite (H7 `2*i+2`).
-Decompose [exchange] H2. Rewrite (H15 i). Rewrite (H15 `2*i+2`).
-Generalize H10. Elim (H5 i); Intros. Exact (H20 H23).
+Decompose [exchange] H2. Rewrite (H16 i). Rewrite (H16 `2*i+2`).
+Generalize H10. Elim (H5 i); Intros. Exact (H21 H24).
 Omega'. Omega'. Omega'. 
 Elim H0; Omega'. Omega'. Omega'. Omega'.
 Elim H0; Omega'. Elim H0; Omega'. 
 Intro. Apply H6; Elim H0; Omega'.
 Save.
 
-Lemma Lemma_2 : (N:Z)(t0,t1,t2:(array N Z))
+Lemma Lemma_2 : (t0,t1,t2:(array Z))
     (n0,k0,j':Z)
     `2*k0+1 <= n0`
  -> (select_son t0 k0 n0 j')
  -> `(access   t0 k0) < (access   t0 j')`
  -> (exchange t1 t0 k0 j')
  -> `0 <= k0 <= n0`
- -> `n0 < N`
+ -> `n0 < (array_length t0)`
  -> ((i:Z)`k0+1 <= i <= n0`->(heap t0 n0 i))
  -> ((i:Z)`j' <= i <= n0`->(heap t2 n0 i))
  -> ((i:Z)
-        `0 <= i < j'`\/`j' < i < 2*j'+1`\/`n0 < i < N`
+        `0 <= i < j'`\/`j' < i < 2*j'+1`\/`n0 < i < (array_length t0)`
         ->`(access   t2 i) = (access   t1 i)`)
  -> ((v:Z)(inftree t1 n0 v j')->(inftree t2 n0 v j'))
  -> (i:Z)`k0 <= i <= n0`->(heap t2 n0 i).
@@ -86,7 +86,7 @@ Elim (Z_lt_ge_dec i j'); Intro HHi.
 Elim (Z_le_lt_eq_dec k0 i); [ Intro HHHi | Intro HHHi | Intuition ].
 
 (* 1. k0 < i < j' *)
-Apply (Lemma_1 N t0 t1 t2 n0 k0 j'); Assumption Orelse Omega'.
+Apply (Lemma_1 t0 t1 t2 n0 k0 j'); Assumption Orelse Omega'.
 
 (* 2. k0 = i *)
 Apply heap_cons.
@@ -96,7 +96,7 @@ Omega'.
 Intro. Elim H0; Intros.
   (* j' = 2k+1 *)
   Rewrite <- HHHi. Rewrite <- H11.
-  Rewrite (H7 k0). Decompose [exchange] H2. Rewrite H15.
+  Rewrite (H7 k0). Decompose [exchange] H2. Rewrite H16.
   Apply Zle_ge. Apply inftree_1 with n:=n0.
   Apply H8.
   Apply inftree_2 with t1:=t0 k:=k0. Omega'. 
@@ -104,26 +104,26 @@ Intro. Elim H0; Intros.
   Apply H5; Omega'. Assumption. Omega'. Omega'. Omega'.
   (* j' = 2k+2 *)
   Rewrite <- HHHi.
-  Rewrite (H7 k0). Decompose [exchange] H2. Rewrite H16.
-  Rewrite (H7 `2*k0+1`). Rewrite (H18 `2*k0+1`).
+  Rewrite (H7 k0). Decompose [exchange] H2. Rewrite H17.
+  Rewrite (H7 `2*k0+1`). Rewrite (H19 `2*k0+1`).
   Omega'. Omega'. Omega'. Omega'. Omega'. Omega'. 
 (* (heap t2 n (2k+1)) *)
 Intro. Elim H0; Intros.
   (* j' = 2k+1 *)
   Apply H6; Omega'.
   (* j' = 2k+2 *)
-  Apply (Lemma_1 N t0 t1 t2 n0 k0 j'); Assumption Orelse Omega'.
+  Apply (Lemma_1 t0 t1 t2 n0 k0 j'); Assumption Orelse Omega'.
 (* branch 2i+2 *)
 (* t[k] >= t[2k+2] *)
 Intro. Elim H0; Intros.
   (* j' = 2k+1 *)
   Rewrite <- HHHi.
-  Rewrite (H7 k0). Decompose [exchange] H2. Rewrite H15.
-  Rewrite (H7 `2*k0+2`). Rewrite (H17 `2*k0+2`).
+  Rewrite (H7 k0). Decompose [exchange] H2. Rewrite H16.
+  Rewrite (H7 `2*k0+2`). Rewrite (H18 `2*k0+2`).
   Omega'. Omega'. Omega'. Omega'. Omega'. Omega'. 
   (* j' = 2k+2 *)
   Rewrite <- HHHi. Rewrite <- H11.
-  Rewrite (H7 k0). Decompose [exchange] H2. Rewrite H16.
+  Rewrite (H7 k0). Decompose [exchange] H2. Rewrite H17.
   Apply Zle_ge. Apply inftree_1 with n:=n0.
   Apply H8.
   Apply inftree_2 with t1:=t0 k:=k0. Omega'. 
@@ -144,68 +144,62 @@ Save.
 (* Obligations *)
 
 Lemma downheap_po_1 : 
-  (N: Z)
   (k: Z)
   (n: Z)
-  (t: (array N Z))
-  (Pre15: (`0 <= k` /\ `k <= n`) /\ `n < N` /\
+  (t: (array Z))
+  (Pre15: (`0 <= k` /\ `k <= n`) /\ `n < (array_length t)` /\
           ((i:Z) (`k + 1 <= i` /\ `i <= n` -> (heap t n i))))
   (Variant1: Z)
-  (N0: Z)
   (k0: Z)
   (n0: Z)
-  (t0: (array N0 Z))
+  (t0: (array Z))
   (Pre14: Variant1 = `n0 - k0`)
-  (Pre13: (`0 <= k0` /\ `k0 <= n0`) /\ `n0 < N0` /\
+  (Pre13: (`0 <= k0` /\ `k0 <= n0`) /\ `n0 < (array_length t0)` /\
           ((i:Z) (`k0 + 1 <= i` /\ `i <= n0` -> (heap t0 n0 i))))
   (j: Z)
   (Post2: j = `2 * k0 + 1`)
   (Test8: `j <= n0`)
   (Test5: `j + 1 <= n0`)
-  `0 <= j + 1` /\ `j + 1 < N0`.
+  `0 <= j + 1` /\ `j + 1 < (array_length t0)`.
 Proof.
 Intros; Omega'.
 Save.
 
 Lemma downheap_po_2 : 
-  (N: Z)
   (k: Z)
   (n: Z)
-  (t: (array N Z))
-  (Pre15: (`0 <= k` /\ `k <= n`) /\ `n < N` /\
+  (t: (array Z))
+  (Pre15: (`0 <= k` /\ `k <= n`) /\ `n < (array_length t)` /\
           ((i:Z) (`k + 1 <= i` /\ `i <= n` -> (heap t n i))))
   (Variant1: Z)
-  (N0: Z)
   (k0: Z)
   (n0: Z)
-  (t0: (array N0 Z))
+  (t0: (array Z))
   (Pre14: Variant1 = `n0 - k0`)
-  (Pre13: (`0 <= k0` /\ `k0 <= n0`) /\ `n0 < N0` /\
+  (Pre13: (`0 <= k0` /\ `k0 <= n0`) /\ `n0 < (array_length t0)` /\
           ((i:Z) (`k0 + 1 <= i` /\ `i <= n0` -> (heap t0 n0 i))))
   (j: Z)
   (Post2: j = `2 * k0 + 1`)
   (Test8: `j <= n0`)
   (Test5: `j + 1 <= n0`)
-  (Pre3: `0 <= j + 1` /\ `j + 1 < N0`)
-  `0 <= j` /\ `j < N0`.
+  (Pre3: `0 <= j + 1` /\ `j + 1 < (array_length t0)`)
+  `0 <= j` /\ `j < (array_length t0)`.
 Proof.
 Intros; Omega'.
 Save.
 
 Lemma downheap_po_3 : 
-  (N: Z)
   (k: Z)
   (n: Z)
-  (t: (array N Z))
-  (Pre15: (`0 <= k` /\ `k <= n`) /\ `n < N` /\
+  (t: (array Z))
+  (Pre15: (`0 <= k` /\ `k <= n`) /\ `n < (array_length t)` /\
           ((i:Z) (`k + 1 <= i` /\ `i <= n` -> (heap t n i))))
   (Variant1: Z)
-  (N0: Z)
   (k0: Z)
   (n0: Z)
-  (t0: (array N0 Z))
+  (t0: (array Z))
   (Pre14: Variant1 = `n0 - k0`)
-  (Pre13: (`0 <= k0` /\ `k0 <= n0`) /\ `n0 < N0` /\
+  (Pre13: (`0 <= k0` /\ `k0 <= n0`) /\ `n0 < (array_length t0)` /\
           ((i:Z) (`k0 + 1 <= i` /\ `i <= n0` -> (heap t0 n0 i))))
   (j: Z)
   (Post2: j = `2 * k0 + 1`)
@@ -221,19 +215,17 @@ Apply select_right_son;
 Save.
 
 Lemma downheap_po_4 : 
-  (N: Z)
   (k: Z)
   (n: Z)
-  (t: (array N Z))
-  (Pre15: (`0 <= k` /\ `k <= n`) /\ `n < N` /\
+  (t: (array Z))
+  (Pre15: (`0 <= k` /\ `k <= n`) /\ `n < (array_length t)` /\
           ((i:Z) (`k + 1 <= i` /\ `i <= n` -> (heap t n i))))
   (Variant1: Z)
-  (N0: Z)
   (k0: Z)
   (n0: Z)
-  (t0: (array N0 Z))
+  (t0: (array Z))
   (Pre14: Variant1 = `n0 - k0`)
-  (Pre13: (`0 <= k0` /\ `k0 <= n0`) /\ `n0 < N0` /\
+  (Pre13: (`0 <= k0` /\ `k0 <= n0`) /\ `n0 < (array_length t0)` /\
           ((i:Z) (`k0 + 1 <= i` /\ `i <= n0` -> (heap t0 n0 i))))
   (j: Z)
   (Post2: j = `2 * k0 + 1`)
@@ -249,19 +241,17 @@ Apply select_left_son;
 Save.
 
 Lemma downheap_po_5 : 
-  (N: Z)
   (k: Z)
   (n: Z)
-  (t: (array N Z))
-  (Pre15: (`0 <= k` /\ `k <= n`) /\ `n < N` /\
+  (t: (array Z))
+  (Pre15: (`0 <= k` /\ `k <= n`) /\ `n < (array_length t)` /\
           ((i:Z) (`k + 1 <= i` /\ `i <= n` -> (heap t n i))))
   (Variant1: Z)
-  (N0: Z)
   (k0: Z)
   (n0: Z)
-  (t0: (array N0 Z))
+  (t0: (array Z))
   (Pre14: Variant1 = `n0 - k0`)
-  (Pre13: (`0 <= k0` /\ `k0 <= n0`) /\ `n0 < N0` /\
+  (Pre13: (`0 <= k0` /\ `k0 <= n0`) /\ `n0 < (array_length t0)` /\
           ((i:Z) (`k0 + 1 <= i` /\ `i <= n0` -> (heap t0 n0 i))))
   (j: Z)
   (Post2: j = `2 * k0 + 1`)
@@ -275,70 +265,64 @@ Apply select_left_son; [ Reflexivity | Intro; Absurd `2*k+2 <= n`; Omega' ].
 Save.
 
 Lemma downheap_po_6 : 
-  (N: Z)
   (k: Z)
   (n: Z)
-  (t: (array N Z))
-  (Pre15: (`0 <= k` /\ `k <= n`) /\ `n < N` /\
+  (t: (array Z))
+  (Pre15: (`0 <= k` /\ `k <= n`) /\ `n < (array_length t)` /\
           ((i:Z) (`k + 1 <= i` /\ `i <= n` -> (heap t n i))))
   (Variant1: Z)
-  (N0: Z)
   (k0: Z)
   (n0: Z)
-  (t0: (array N0 Z))
+  (t0: (array Z))
   (Pre14: Variant1 = `n0 - k0`)
-  (Pre13: (`0 <= k0` /\ `k0 <= n0`) /\ `n0 < N0` /\
+  (Pre13: (`0 <= k0` /\ `k0 <= n0`) /\ `n0 < (array_length t0)` /\
           ((i:Z) (`k0 + 1 <= i` /\ `i <= n0` -> (heap t0 n0 i))))
   (j: Z)
   (Post2: j = `2 * k0 + 1`)
   (Test8: `j <= n0`)
   (j': Z)
   (Post11: (select_son t0 k0 n0 j'))
-  `0 <= j'` /\ `j' < N0`.
+  `0 <= j'` /\ `j' < (array_length t0)`.
 Proof.
 Intros; Elim Post11; Intros; Omega'.
 Save.
 
 Lemma downheap_po_7 : 
-  (N: Z)
   (k: Z)
   (n: Z)
-  (t: (array N Z))
-  (Pre15: (`0 <= k` /\ `k <= n`) /\ `n < N` /\
+  (t: (array Z))
+  (Pre15: (`0 <= k` /\ `k <= n`) /\ `n < (array_length t)` /\
           ((i:Z) (`k + 1 <= i` /\ `i <= n` -> (heap t n i))))
   (Variant1: Z)
-  (N0: Z)
   (k0: Z)
   (n0: Z)
-  (t0: (array N0 Z))
+  (t0: (array Z))
   (Pre14: Variant1 = `n0 - k0`)
-  (Pre13: (`0 <= k0` /\ `k0 <= n0`) /\ `n0 < N0` /\
+  (Pre13: (`0 <= k0` /\ `k0 <= n0`) /\ `n0 < (array_length t0)` /\
           ((i:Z) (`k0 + 1 <= i` /\ `i <= n0` -> (heap t0 n0 i))))
   (j: Z)
   (Post2: j = `2 * k0 + 1`)
   (Test8: `j <= n0`)
   (j': Z)
   (Post11: (select_son t0 k0 n0 j'))
-  (Pre5: `0 <= j'` /\ `j' < N0`)
-  `0 <= k0` /\ `k0 < N0`.
+  (Pre5: `0 <= j'` /\ `j' < (array_length t0)`)
+  `0 <= k0` /\ `k0 < (array_length t0)`.
 Proof.
 Intros; Omega'.
 Save.
 
 Lemma downheap_po_8 : 
-  (N: Z)
   (k: Z)
   (n: Z)
-  (t: (array N Z))
-  (Pre15: (`0 <= k` /\ `k <= n`) /\ `n < N` /\
+  (t: (array Z))
+  (Pre15: (`0 <= k` /\ `k <= n`) /\ `n < (array_length t)` /\
           ((i:Z) (`k + 1 <= i` /\ `i <= n` -> (heap t n i))))
   (Variant1: Z)
-  (N0: Z)
   (k0: Z)
   (n0: Z)
-  (t0: (array N0 Z))
+  (t0: (array Z))
   (Pre14: Variant1 = `n0 - k0`)
-  (Pre13: (`0 <= k0` /\ `k0 <= n0`) /\ `n0 < N0` /\
+  (Pre13: (`0 <= k0` /\ `k0 <= n0`) /\ `n0 < (array_length t0)` /\
           ((i:Z) (`k0 + 1 <= i` /\ `i <= n0` -> (heap t0 n0 i))))
   (j: Z)
   (Post2: j = `2 * k0 + 1`)
@@ -346,25 +330,24 @@ Lemma downheap_po_8 :
   (j': Z)
   (Post11: (select_son t0 k0 n0 j'))
   (Test7: `(access t0 k0) < (access t0 j')`)
-  (`0 <= k0` /\ `k0 < N0`) /\ `0 <= j'` /\ `j' < N0`.
+  (`0 <= k0` /\ `k0 < (array_length t0)`) /\ `0 <= j'` /\
+  `j' < (array_length t0)`.
 Proof.
 Intros; Elim Post11; Intros; Omega'.
 Save.
 
 Lemma downheap_po_9 : 
-  (N: Z)
   (k: Z)
   (n: Z)
-  (t: (array N Z))
-  (Pre15: (`0 <= k` /\ `k <= n`) /\ `n < N` /\
+  (t: (array Z))
+  (Pre15: (`0 <= k` /\ `k <= n`) /\ `n < (array_length t)` /\
           ((i:Z) (`k + 1 <= i` /\ `i <= n` -> (heap t n i))))
   (Variant1: Z)
-  (N0: Z)
   (k0: Z)
   (n0: Z)
-  (t0: (array N0 Z))
+  (t0: (array Z))
   (Pre14: Variant1 = `n0 - k0`)
-  (Pre13: (`0 <= k0` /\ `k0 <= n0`) /\ `n0 < N0` /\
+  (Pre13: (`0 <= k0` /\ `k0 <= n0`) /\ `n0 < (array_length t0)` /\
           ((i:Z) (`k0 + 1 <= i` /\ `i <= n0` -> (heap t0 n0 i))))
   (j: Z)
   (Post2: j = `2 * k0 + 1`)
@@ -372,34 +355,33 @@ Lemma downheap_po_9 :
   (j': Z)
   (Post11: (select_son t0 k0 n0 j'))
   (Test7: `(access t0 k0) < (access t0 j')`)
-  (Pre12: (`0 <= k0` /\ `k0 < N0`) /\ `0 <= j'` /\ `j' < N0`)
-  (t1: (array N0 Z))
+  (Pre12: (`0 <= k0` /\ `k0 < (array_length t0)`) /\ `0 <= j'` /\
+          `j' < (array_length t0)`)
+  (t1: (array Z))
   (Post22: (exchange t1 t0 k0 j'))
-  (`0 <= j'` /\ `j' <= n0`) /\ `n0 < N0` /\
+  (`0 <= j'` /\ `j' <= n0`) /\ `n0 < (array_length t1)` /\
   ((i:Z) (`j' + 1 <= i` /\ `i <= n0` -> (heap t1 n0 i))).
 Proof.
-Intuition; Try (Elim Post11; Omega').
+Intuition; Try (Elim Post11; SameLength t1 t0; Omega').
 Apply heap_id with t := t0.
 Apply H7; Elim Post11; Omega'.
 Unfold array_id. Intros i' Hi'.
 Elim Post22; Intros.
-Symmetry; Apply (H17 i'); Elim Post11; Omega'.
+Symmetry; Apply (H18 i'); Elim Post11; Omega'.
 Save.
 
 Lemma downheap_po_10 : 
-  (N: Z)
   (k: Z)
   (n: Z)
-  (t: (array N Z))
-  (Pre15: (`0 <= k` /\ `k <= n`) /\ `n < N` /\
+  (t: (array Z))
+  (Pre15: (`0 <= k` /\ `k <= n`) /\ `n < (array_length t)` /\
           ((i:Z) (`k + 1 <= i` /\ `i <= n` -> (heap t n i))))
   (Variant1: Z)
-  (N0: Z)
   (k0: Z)
   (n0: Z)
-  (t0: (array N0 Z))
+  (t0: (array Z))
   (Pre14: Variant1 = `n0 - k0`)
-  (Pre13: (`0 <= k0` /\ `k0 <= n0`) /\ `n0 < N0` /\
+  (Pre13: (`0 <= k0` /\ `k0 <= n0`) /\ `n0 < (array_length t0)` /\
           ((i:Z) (`k0 + 1 <= i` /\ `i <= n0` -> (heap t0 n0 i))))
   (j: Z)
   (Post2: j = `2 * k0 + 1`)
@@ -407,14 +389,15 @@ Lemma downheap_po_10 :
   (j': Z)
   (Post11: (select_son t0 k0 n0 j'))
   (Test7: `(access t0 k0) < (access t0 j')`)
-  (Pre12: (`0 <= k0` /\ `k0 < N0`) /\ `0 <= j'` /\ `j' < N0`)
-  (t1: (array N0 Z))
+  (Pre12: (`0 <= k0` /\ `k0 < (array_length t0)`) /\ `0 <= j'` /\
+          `j' < (array_length t0)`)
+  (t1: (array Z))
   (Post22: (exchange t1 t0 k0 j'))
-  (Pre11: (`0 <= j'` /\ `j' <= n0`) /\ `n0 < N0` /\
+  (Pre11: (`0 <= j'` /\ `j' <= n0`) /\ `n0 < (array_length t1)` /\
           ((i:Z) (`j' + 1 <= i` /\ `i <= n0` -> (heap t1 n0 i))))
-  (Pre9: (`0 <= j'` /\ `j' <= n0`) /\ `n0 < N0` /\
+  (Pre9: (`0 <= j'` /\ `j' <= n0`) /\ `n0 < (array_length t1)` /\
          ((i:Z) (`j' + 1 <= i` /\ `i <= n0` -> (heap t1 n0 i))))
-  (Pre10: (`0 <= j'` /\ `j' <= n0`) /\ `n0 < N0` /\
+  (Pre10: (`0 <= j'` /\ `j' <= n0`) /\ `n0 < (array_length t1)` /\
           ((i:Z) (`j' + 1 <= i` /\ `i <= n0` -> (heap t1 n0 i))))
   (Zwf `0` `n0 - j'` Variant1).
 Proof.
@@ -422,19 +405,17 @@ Intros; Unfold Zwf; Decompose [select_son] Post11; Omega'.
 Save.
 
 Lemma downheap_po_11 : 
-  (N: Z)
   (k: Z)
   (n: Z)
-  (t: (array N Z))
-  (Pre15: (`0 <= k` /\ `k <= n`) /\ `n < N` /\
+  (t: (array Z))
+  (Pre15: (`0 <= k` /\ `k <= n`) /\ `n < (array_length t)` /\
           ((i:Z) (`k + 1 <= i` /\ `i <= n` -> (heap t n i))))
   (Variant1: Z)
-  (N0: Z)
   (k0: Z)
   (n0: Z)
-  (t0: (array N0 Z))
+  (t0: (array Z))
   (Pre14: Variant1 = `n0 - k0`)
-  (Pre13: (`0 <= k0` /\ `k0 <= n0`) /\ `n0 < N0` /\
+  (Pre13: (`0 <= k0` /\ `k0 <= n0`) /\ `n0 < (array_length t0)` /\
           ((i:Z) (`k0 + 1 <= i` /\ `i <= n0` -> (heap t0 n0 i))))
   (j: Z)
   (Post2: j = `2 * k0 + 1`)
@@ -442,35 +423,34 @@ Lemma downheap_po_11 :
   (j': Z)
   (Post11: (select_son t0 k0 n0 j'))
   (Test7: `(access t0 k0) < (access t0 j')`)
-  (Pre12: (`0 <= k0` /\ `k0 < N0`) /\ `0 <= j'` /\ `j' < N0`)
-  (t1: (array N0 Z))
+  (Pre12: (`0 <= k0` /\ `k0 < (array_length t0)`) /\ `0 <= j'` /\
+          `j' < (array_length t0)`)
+  (t1: (array Z))
   (Post22: (exchange t1 t0 k0 j'))
-  (Pre11: (`0 <= j'` /\ `j' <= n0`) /\ `n0 < N0` /\
+  (Pre11: (`0 <= j'` /\ `j' <= n0`) /\ `n0 < (array_length t1)` /\
           ((i:Z) (`j' + 1 <= i` /\ `i <= n0` -> (heap t1 n0 i))))
-  (Pre9: (`0 <= j'` /\ `j' <= n0`) /\ `n0 < N0` /\
+  (Pre9: (`0 <= j'` /\ `j' <= n0`) /\ `n0 < (array_length t1)` /\
          ((i:Z) (`j' + 1 <= i` /\ `i <= n0` -> (heap t1 n0 i))))
-  (Pre10: (`0 <= j'` /\ `j' <= n0`) /\ `n0 < N0` /\
+  (Pre10: (`0 <= j'` /\ `j' <= n0`) /\ `n0 < (array_length t1)` /\
           ((i:Z) (`j' + 1 <= i` /\ `i <= n0` -> (heap t1 n0 i))))
-  (`0 <= j'` /\ `j' <= n0`) /\ `n0 < N0` /\
+  (`0 <= j'` /\ `j' <= n0`) /\ `n0 < (array_length t1)` /\
   ((i:Z) (`j' + 1 <= i` /\ `i <= n0` -> (heap t1 n0 i))).
 Proof.
 Intuition.
 Save.
 
 Lemma downheap_po_12 : 
-  (N: Z)
   (k: Z)
   (n: Z)
-  (t: (array N Z))
-  (Pre15: (`0 <= k` /\ `k <= n`) /\ `n < N` /\
+  (t: (array Z))
+  (Pre15: (`0 <= k` /\ `k <= n`) /\ `n < (array_length t)` /\
           ((i:Z) (`k + 1 <= i` /\ `i <= n` -> (heap t n i))))
   (Variant1: Z)
-  (N0: Z)
   (k0: Z)
   (n0: Z)
-  (t0: (array N0 Z))
+  (t0: (array Z))
   (Pre14: Variant1 = `n0 - k0`)
-  (Pre13: (`0 <= k0` /\ `k0 <= n0`) /\ `n0 < N0` /\
+  (Pre13: (`0 <= k0` /\ `k0 <= n0`) /\ `n0 < (array_length t0)` /\
           ((i:Z) (`k0 + 1 <= i` /\ `i <= n0` -> (heap t0 n0 i))))
   (j: Z)
   (Post2: j = `2 * k0 + 1`)
@@ -478,22 +458,24 @@ Lemma downheap_po_12 :
   (j': Z)
   (Post11: (select_son t0 k0 n0 j'))
   (Test7: `(access t0 k0) < (access t0 j')`)
-  (Pre12: (`0 <= k0` /\ `k0 < N0`) /\ `0 <= j'` /\ `j' < N0`)
-  (t1: (array N0 Z))
+  (Pre12: (`0 <= k0` /\ `k0 < (array_length t0)`) /\ `0 <= j'` /\
+          `j' < (array_length t0)`)
+  (t1: (array Z))
   (Post22: (exchange t1 t0 k0 j'))
-  (Pre11: (`0 <= j'` /\ `j' <= n0`) /\ `n0 < N0` /\
+  (Pre11: (`0 <= j'` /\ `j' <= n0`) /\ `n0 < (array_length t1)` /\
           ((i:Z) (`j' + 1 <= i` /\ `i <= n0` -> (heap t1 n0 i))))
-  (t2: (array N0 Z))
+  (t2: (array Z))
   (Post24: (permut t2 t1) /\
            ((i:Z) (`j' <= i` /\ `i <= n0` -> (heap t2 n0 i))) /\
            ((i:Z)
             (`0 <= i` /\ `i < j'` \/ `j' < i` /\ `i < 2 * j' + 1` \/
-             `n0 < i` /\ `i < N0` -> `(access t2 i) = (access t1 i)`)) /\
+             `n0 < i` /\ `i < (array_length t2)` ->
+             `(access t2 i) = (access t1 i)`)) /\
            ((v:Z) ((inftree t1 n0 v j') -> (inftree t2 n0 v j'))))
   (permut t2 t0) /\ ((i:Z) (`k0 <= i` /\ `i <= n0` -> (heap t2 n0 i))) /\
   ((i:Z)
    (`0 <= i` /\ `i < k0` \/ `k0 < i` /\ `i < 2 * k0 + 1` \/ `n0 < i` /\
-    `i < N0` -> `(access t2 i) = (access t0 i)`)) /\
+    `i < (array_length t2)` -> `(access t2 i) = (access t0 i)`)) /\
   ((v:Z) ((inftree t0 n0 v k0) -> (inftree t2 n0 v k0))).
 Proof.
 Intuition.
@@ -502,28 +484,30 @@ Intuition.
 Apply permut_trans with t' := t1.
 Intuition. Apply exchange_is_permut with i:=k0 j:=j'; Assumption.
 (* heap *)
-Apply (Lemma_2 N0 t0 t1 t2 n0 k0 j'); Assumption Orelse Omega'.
+Apply (Lemma_2 t0 t1 t2 n0 k0 j'); Assumption Orelse Try Omega'.
+SameLength t2 t1. SameLength t1 t0.
+Rewrite <- H22; Rewrite <- H18; Assumption.
 (* unchanged parts of the array *)
 Rewrite (H16 i);
-[ Decompose [exchange] Post22; Apply H25 | Idtac ];
+[ Decompose [exchange] Post22; Apply H26 | Idtac ];
 Decompose [select_son] Post11; Omega'.
 Rewrite (H16 i); 
-[ Decompose [exchange] Post22; Apply H25 | Idtac ];
+[ Decompose [exchange] Post22; Apply H26 | Idtac ];
 Decompose [select_son] Post11; Omega'.
 Rewrite (H16 i); 
-[ Decompose [exchange] Post22; Apply H25 | Idtac ];
-Decompose [select_son] Post11; Omega'.
+[ Decompose [exchange] Post22; Apply H26 | Idtac ];
+Decompose [select_son] Post11; SameLength t2 t1; Omega'.
 (* inftree *)
 Apply inftree_cons.
 Split; Assumption.
 Rewrite (H16 k0). 
-Decompose [exchange] Post22. Rewrite H22. 
+Decompose [exchange] Post22. Rewrite H23. 
 Elim Post11; Intros.
   (* j' = 2k+1 *)
-  Rewrite H25. Generalize Test8; Rewrite Post2. Case H18; Intros.
+  Rewrite H26. Generalize Test8; Rewrite Post2. Case H18; Intros.
   Apply inftree_1 with n:=n0. Auto.
   (* j' = 2k+2 *)
-  Generalize H26. Rewrite H25. Case H18; Intros.
+  Generalize H27. Rewrite H26. Case H18; Intros.
   Apply inftree_1 with n:=n0. Auto.
 Elim Post11; Intros; Omega'.
   (* branch 2k+1 *)
@@ -536,18 +520,21 @@ Elim Post11; Intros; Omega'.
     (* j' = 2k+2 *)
     Apply inftree_trans with v:=#t2[`2*k0+1`].
     Rewrite (H16 `2*k0+1`).
-    Decompose [exchange] Post22. Rewrite (H28 `2*k0+1`).
+    Decompose [exchange] Post22. Rewrite (H29 `2*k0+1`).
     Generalize H20. Case H18; Intros.
     Apply inftree_1 with n:=n0. Auto.
     Omega'. Omega'. Omega'. Omega'.
     Apply inftree_3.
-    Apply (Lemma_2 N0 t0 t1 t2 n0 k0 j'); Assumption Orelse Omega'.
+    Apply (Lemma_2 t0 t1 t2 n0 k0 j'); Assumption Orelse Try Omega'.
+    SameLength t2 t1. SameLength t1 t0.
+    Rewrite <- H25; Rewrite <- H24; Assumption.
+
   (* branch 2k+2 *)
   Intro. Elim Post11; Intros.
     (* j' = 2k+1 *)
     Apply inftree_trans with v:=#t2[`2*k0+2`].
     Rewrite (H16 `2*k0+2`).
-    Decompose [exchange] Post22. Rewrite (H27 `2*k0+2`).
+    Decompose [exchange] Post22. Rewrite (H28 `2*k0+2`).
     Generalize H20. Case H18; Intros.
     Apply inftree_1 with n:=n0. Auto.
     Omega'. Omega'. Omega'. Omega'.
@@ -561,19 +548,17 @@ Elim Post11; Intros; Omega'.
 Save.
 
 Lemma downheap_po_13 : 
-  (N: Z)
   (k: Z)
   (n: Z)
-  (t: (array N Z))
-  (Pre15: (`0 <= k` /\ `k <= n`) /\ `n < N` /\
+  (t: (array Z))
+  (Pre15: (`0 <= k` /\ `k <= n`) /\ `n < (array_length t)` /\
           ((i:Z) (`k + 1 <= i` /\ `i <= n` -> (heap t n i))))
   (Variant1: Z)
-  (N0: Z)
   (k0: Z)
   (n0: Z)
-  (t0: (array N0 Z))
+  (t0: (array Z))
   (Pre14: Variant1 = `n0 - k0`)
-  (Pre13: (`0 <= k0` /\ `k0 <= n0`) /\ `n0 < N0` /\
+  (Pre13: (`0 <= k0` /\ `k0 <= n0`) /\ `n0 < (array_length t0)` /\
           ((i:Z) (`k0 + 1 <= i` /\ `i <= n0` -> (heap t0 n0 i))))
   (j: Z)
   (Post2: j = `2 * k0 + 1`)
@@ -584,7 +569,7 @@ Lemma downheap_po_13 :
   (permut t0 t0) /\ ((i:Z) (`k0 <= i` /\ `i <= n0` -> (heap t0 n0 i))) /\
   ((i:Z)
    (`0 <= i` /\ `i < k0` \/ `k0 < i` /\ `i < 2 * k0 + 1` \/ `n0 < i` /\
-    `i < N0` -> `(access t0 i) = (access t0 i)`)) /\
+    `i < (array_length t0)` -> `(access t0 i) = (access t0 i)`)) /\
   ((v:Z) ((inftree t0 n0 v k0) -> (inftree t0 n0 v k0))).
 Proof.
 Intuition.
@@ -603,19 +588,17 @@ Intro. Apply H7; Omega'.
 Save.
 
 Lemma downheap_po_14 : 
-  (N: Z)
   (k: Z)
   (n: Z)
-  (t: (array N Z))
-  (Pre15: (`0 <= k` /\ `k <= n`) /\ `n < N` /\
+  (t: (array Z))
+  (Pre15: (`0 <= k` /\ `k <= n`) /\ `n < (array_length t)` /\
           ((i:Z) (`k + 1 <= i` /\ `i <= n` -> (heap t n i))))
   (Variant1: Z)
-  (N0: Z)
   (k0: Z)
   (n0: Z)
-  (t0: (array N0 Z))
+  (t0: (array Z))
   (Pre14: Variant1 = `n0 - k0`)
-  (Pre13: (`0 <= k0` /\ `k0 <= n0`) /\ `n0 < N0` /\
+  (Pre13: (`0 <= k0` /\ `k0 <= n0`) /\ `n0 < (array_length t0)` /\
           ((i:Z) (`k0 + 1 <= i` /\ `i <= n0` -> (heap t0 n0 i))))
   (j: Z)
   (Post2: j = `2 * k0 + 1`)
@@ -623,7 +606,7 @@ Lemma downheap_po_14 :
   (permut t0 t0) /\ ((i:Z) (`k0 <= i` /\ `i <= n0` -> (heap t0 n0 i))) /\
   ((i:Z)
    (`0 <= i` /\ `i < k0` \/ `k0 < i` /\ `i < 2 * k0 + 1` \/ `n0 < i` /\
-    `i < N0` -> `(access t0 i) = (access t0 i)`)) /\
+    `i < (array_length t0)` -> `(access t0 i) = (access t0 i)`)) /\
   ((v:Z) ((inftree t0 n0 v k0) -> (inftree t0 n0 v k0))).
 Proof.
 Intuition.
@@ -640,32 +623,31 @@ Save.
 Require swap_why.
 
 Definition downheap := (* validation *)
-  [N: Z; k: Z; n: Z; t: (array N Z); Pre15: (`0 <= k` /\ `k <= n`) /\
-   `n < N` /\ ((i:Z) (`k + 1 <= i` /\ `i <= n` -> (heap t n i)))]
+  [k: Z; n: Z; t: (array Z); Pre15: (`0 <= k` /\ `k <= n`) /\
+   `n < (array_length t)` /\
+   ((i:Z) (`k + 1 <= i` /\ `i <= n` -> (heap t n i)))]
     (well_founded_induction Z (Zwf ZERO) (Zwf_well_founded `0`) [Variant1: Z]
-      (N0: Z)(k0: Z)(n0: Z)(t0: (array N0 Z))(_: Variant1 = `n0 - k0`)
-      (_0: (`0 <= k0` /\ `k0 <= n0`) /\ `n0 < N0` /\
+      (k0: Z)(n0: Z)(t0: (array Z))(_: Variant1 = `n0 - k0`)
+      (_0: (`0 <= k0` /\ `k0 <= n0`) /\ `n0 < (array_length t0)` /\
       ((i:Z) (`k0 + 1 <= i` /\ `i <= n0` -> (heap t0 n0 i))))
-      (sig_2 (array N0 Z) unit [t1: (array N0 Z)][result: unit]
-       ((permut t1 t0) /\
+      (sig_2 (array Z) unit [t1: (array Z)][result: unit]((permut t1 t0) /\
        ((i:Z) (`k0 <= i` /\ `i <= n0` -> (heap t1 n0 i))) /\
        ((i:Z)
         (`0 <= i` /\ `i < k0` \/ `k0 < i` /\ `i < 2 * k0 + 1` \/ `n0 < i` /\
-         `i < N0` -> `(access t1 i) = (access t0 i)`)) /\
+         `i < (array_length t1)` -> `(access t1 i) = (access t0 i)`)) /\
        ((v:Z) ((inftree t0 n0 v k0) -> (inftree t1 n0 v k0)))))
       [Variant1: Z; wf1: (Variant2: Z)(Pre1: (Zwf `0` Variant2 Variant1))
-       (N0: Z)(k0: Z)(n0: Z)(t0: (array N0 Z))(_: Variant2 = `n0 - k0`)
-       (_0: (`0 <= k0` /\ `k0 <= n0`) /\ `n0 < N0` /\
+       (k0: Z)(n0: Z)(t0: (array Z))(_: Variant2 = `n0 - k0`)
+       (_0: (`0 <= k0` /\ `k0 <= n0`) /\ `n0 < (array_length t0)` /\
        ((i:Z) (`k0 + 1 <= i` /\ `i <= n0` -> (heap t0 n0 i))))
-       (sig_2 (array N0 Z) unit [t1: (array N0 Z)][result: unit]
-        ((permut t1 t0) /\
+       (sig_2 (array Z) unit [t1: (array Z)][result: unit]((permut t1 t0) /\
         ((i:Z) (`k0 <= i` /\ `i <= n0` -> (heap t1 n0 i))) /\
         ((i:Z)
          (`0 <= i` /\ `i < k0` \/ `k0 < i` /\ `i < 2 * k0 + 1` \/ `n0 < i` /\
-          `i < N0` -> `(access t1 i) = (access t0 i)`)) /\
+          `i < (array_length t1)` -> `(access t1 i) = (access t0 i)`)) /\
         ((v:Z) ((inftree t0 n0 v k0) -> (inftree t1 n0 v k0)))));
-       N0: Z; k0: Z; n0: Z; t0: (array N0 Z); Pre14: Variant1 = `n0 - k0`;
-       Pre13: (`0 <= k0` /\ `k0 <= n0`) /\ `n0 < N0` /\
+       k0: Z; n0: Z; t0: (array Z); Pre14: Variant1 = `n0 - k0`;
+       Pre13: (`0 <= k0` /\ `k0 <= n0`) /\ `n0 < (array_length t0)` /\
        ((i:Z) (`k0 + 1 <= i` /\ `i <= n0` -> (heap t0 n0 i)))]
         let (j, Post2) = (exist_1 [result: Z]
           result = `2 * k0 + 1` `2 * k0 + 1` (refl_equal ? `2 * k0 + 1`)) in
@@ -692,12 +674,12 @@ Definition downheap := (* validation *)
                       let (result1, Post14) =
                         let (result1, Bool5) =
                           let Pre3 =
-                            (downheap_po_1 N k n t Pre15 Variant1 N0 k0 n0 t0
+                            (downheap_po_1 k n t Pre15 Variant1 k0 n0 t0
                             Pre14 Pre13 j Post2 Test8 Test5) in
                           let result2 =
                             let Pre2 =
-                              (downheap_po_2 N k n t Pre15 Variant1 N0 k0 n0
-                              t0 Pre14 Pre13 j Post2 Test8 Test5 Pre3) in
+                              (downheap_po_2 k n t Pre15 Variant1 k0 n0 t0
+                              Pre14 Pre13 j Post2 Test8 Test5 Pre3) in
                             (Z_lt_ge_bool (access t0 j)) in
                           let (result3, Post15) =
                             (result2 (access t0 `j + 1`)) in
@@ -716,15 +698,15 @@ Definition downheap := (* validation *)
                         | (left Test4) =>
                             let (result2, Post17) = (exist_1 [result2: Z]
                               (select_son t0 k0 n0 result2) `j + 1`
-                              (downheap_po_3 N k n t Pre15 Variant1 N0 k0 n0
-                              t0 Pre14 Pre13 j Post2 Test8 Test5 Test4)) in
+                              (downheap_po_3 k n t Pre15 Variant1 k0 n0 t0
+                              Pre14 Pre13 j Post2 Test8 Test5 Test4)) in
                             (exist_1 [result3: Z]
                             (select_son t0 k0 n0 result3) result2 Post17)
                         | (right Test3) =>
                             let (result2, Post16) = (exist_1 [result2: Z]
                               (select_son t0 k0 n0 result2) j
-                              (downheap_po_4 N k n t Pre15 Variant1 N0 k0 n0
-                              t0 Pre14 Pre13 j Post2 Test8 Test5 Test3)) in
+                              (downheap_po_4 k n t Pre15 Variant1 k0 n0 t0
+                              Pre14 Pre13 j Post2 Test8 Test5 Test3)) in
                             (exist_1 [result3: Z]
                             (select_son t0 k0 n0 result3) result2 Post16) end) in
                       (exist_1 [result2: Z]
@@ -732,19 +714,19 @@ Definition downheap := (* validation *)
                   | (right Test2) =>
                       let (result1, Post13) = (exist_1 [result1: Z]
                         (select_son t0 k0 n0 result1) j
-                        (downheap_po_5 N k n t Pre15 Variant1 N0 k0 n0 t0
-                        Pre14 Pre13 j Post2 Test8 Test2)) in
+                        (downheap_po_5 k n t Pre15 Variant1 k0 n0 t0 Pre14
+                        Pre13 j Post2 Test8 Test2)) in
                       (exist_1 [result2: Z]
                       (select_son t0 k0 n0 result2) result1 Post13) end) in
                 let (t1, result0, Post18) =
                   let (result0, Bool7) =
                     let Pre5 =
-                      (downheap_po_6 N k n t Pre15 Variant1 N0 k0 n0 t0 Pre14
+                      (downheap_po_6 k n t Pre15 Variant1 k0 n0 t0 Pre14
                       Pre13 j Post2 Test8 j' Post11) in
                     let result1 =
                       let Pre4 =
-                        (downheap_po_7 N k n t Pre15 Variant1 N0 k0 n0 t0
-                        Pre14 Pre13 j Post2 Test8 j' Post11 Pre5) in
+                        (downheap_po_7 k n t Pre15 Variant1 k0 n0 t0 Pre14
+                        Pre13 j Post2 Test8 j' Post11 Pre5) in
                       (Z_lt_ge_bool (access t0 k0)) in
                     let (result2, Post19) = (result1 (access t0 j')) in
                     (exist_1 [result3: bool]
@@ -761,59 +743,61 @@ Definition downheap := (* validation *)
                   | (left Test7) =>
                       let (t1, result1, Post21) =
                         let Pre12 =
-                          (downheap_po_8 N k n t Pre15 Variant1 N0 k0 n0 t0
-                          Pre14 Pre13 j Post2 Test8 j' Post11 Test7) in
+                          (downheap_po_8 k n t Pre15 Variant1 k0 n0 t0 Pre14
+                          Pre13 j Post2 Test8 j' Post11 Test7) in
                         let (t1, result1, Post22) =
                           let Pre6 = Pre12 in
                           let Pre7 = Pre6 in
-                          let (t1, result3, Post23) =
-                            (swap N0 k0 j' t0 Pre6) in
-                          (exist_2 [t2: (array N0 Z)][result4: unit]
+                          let (t1, result3, Post23) = (swap k0 j' t0 Pre6) in
+                          (exist_2 [t2: (array Z)][result4: unit]
                           (exchange t2 t0 k0 j') t1 result3 Post23) in
                         let Pre11 =
-                          (downheap_po_9 N k n t Pre15 Variant1 N0 k0 n0 t0
-                          Pre14 Pre13 j Post2 Test8 j' Post11 Test7 Pre12 t1
+                          (downheap_po_9 k n t Pre15 Variant1 k0 n0 t0 Pre14
+                          Pre13 j Post2 Test8 j' Post11 Test7 Pre12 t1
                           Post22) in
                         let (t2, result2, Post24) =
                           let Pre9 = Pre11 in
                           let Pre10 = Pre9 in
                           let (t2, result4, Post25) =
                             ((wf1 `n0 - j'`)
-                              (downheap_po_10 N k n t Pre15 Variant1 N0 k0 n0
-                              t0 Pre14 Pre13 j Post2 Test8 j' Post11 Test7
-                              Pre12 t1 Post22 Pre11 Pre9 Pre10) N0 j' 
-                              n0 t1 (refl_equal ? `n0 - j'`)
-                              (downheap_po_11 N k n t Pre15 Variant1 N0 k0 n0
-                              t0 Pre14 Pre13 j Post2 Test8 j' Post11 Test7
-                              Pre12 t1 Post22 Pre11 Pre9 Pre10)) in
-                          (exist_2 [t3: (array N0 Z)][result5: unit]
+                              (downheap_po_10 k n t Pre15 Variant1 k0 n0 t0
+                              Pre14 Pre13 j Post2 Test8 j' Post11 Test7 Pre12
+                              t1 Post22 Pre11 Pre9 Pre10) j' n0 t1
+                              (refl_equal ? `n0 - j'`)
+                              (downheap_po_11 k n t Pre15 Variant1 k0 n0 t0
+                              Pre14 Pre13 j Post2 Test8 j' Post11 Test7 Pre12
+                              t1 Post22 Pre11 Pre9 Pre10)) in
+                          (exist_2 [t3: (array Z)][result5: unit]
                           (permut t3 t1) /\
                           ((i:Z) (`j' <= i` /\ `i <= n0` -> (heap t3 n0 i))) /\
                           ((i:Z)
                            (`0 <= i` /\ `i < j'` \/ `j' < i` /\
-                            `i < 2 * j' + 1` \/ `n0 < i` /\ `i < N0` ->
+                            `i < 2 * j' + 1` \/ `n0 < i` /\
+                            `i < (array_length t3)` ->
                             `(access t3 i) = (access t1 i)`)) /\
                           ((v:Z)
                            ((inftree t1 n0 v j') -> (inftree t3 n0 v j'))) 
                           t2 result4 Post25) in
-                        (exist_2 [t3: (array N0 Z)][result3: unit]
+                        (exist_2 [t3: (array Z)][result3: unit]
                         (permut t3 t0) /\
                         ((i:Z) (`k0 <= i` /\ `i <= n0` -> (heap t3 n0 i))) /\
                         ((i:Z)
                          (`0 <= i` /\ `i < k0` \/ `k0 < i` /\
-                          `i < 2 * k0 + 1` \/ `n0 < i` /\ `i < N0` ->
+                          `i < 2 * k0 + 1` \/ `n0 < i` /\
+                          `i < (array_length t3)` ->
                           `(access t3 i) = (access t0 i)`)) /\
                         ((v:Z) ((inftree t0 n0 v k0) -> (inftree t3 n0 v k0))) 
                         t2 result2
-                        (downheap_po_12 N k n t Pre15 Variant1 N0 k0 n0 t0
-                        Pre14 Pre13 j Post2 Test8 j' Post11 Test7 Pre12 t1
-                        Post22 Pre11 t2 Post24)) in
-                      (exist_2 [t2: (array N0 Z)][result2: unit]
+                        (downheap_po_12 k n t Pre15 Variant1 k0 n0 t0 Pre14
+                        Pre13 j Post2 Test8 j' Post11 Test7 Pre12 t1 Post22
+                        Pre11 t2 Post24)) in
+                      (exist_2 [t2: (array Z)][result2: unit]
                       (permut t2 t0) /\
                       ((i:Z) (`k0 <= i` /\ `i <= n0` -> (heap t2 n0 i))) /\
                       ((i:Z)
                        (`0 <= i` /\ `i < k0` \/ `k0 < i` /\
-                        `i < 2 * k0 + 1` \/ `n0 < i` /\ `i < N0` ->
+                        `i < 2 * k0 + 1` \/ `n0 < i` /\
+                        `i < (array_length t2)` ->
                         `(access t2 i) = (access t0 i)`)) /\
                       ((v:Z) ((inftree t0 n0 v k0) -> (inftree t2 n0 v k0))) 
                       t1 result1 Post21)
@@ -823,33 +807,37 @@ Definition downheap := (* validation *)
                         ((i:Z) (`k0 <= i` /\ `i <= n0` -> (heap t0 n0 i))) /\
                         ((i:Z)
                          (`0 <= i` /\ `i < k0` \/ `k0 < i` /\
-                          `i < 2 * k0 + 1` \/ `n0 < i` /\ `i < N0` ->
+                          `i < 2 * k0 + 1` \/ `n0 < i` /\
+                          `i < (array_length t0)` ->
                           `(access t0 i) = (access t0 i)`)) /\
                         ((v:Z) ((inftree t0 n0 v k0) -> (inftree t0 n0 v k0))) 
                         tt
-                        (downheap_po_13 N k n t Pre15 Variant1 N0 k0 n0 t0
-                        Pre14 Pre13 j Post2 Test8 j' Post11 Test6)) in
-                      (exist_2 [t1: (array N0 Z)][result2: unit]
+                        (downheap_po_13 k n t Pre15 Variant1 k0 n0 t0 Pre14
+                        Pre13 j Post2 Test8 j' Post11 Test6)) in
+                      (exist_2 [t1: (array Z)][result2: unit]
                       (permut t1 t0) /\
                       ((i:Z) (`k0 <= i` /\ `i <= n0` -> (heap t1 n0 i))) /\
                       ((i:Z)
                        (`0 <= i` /\ `i < k0` \/ `k0 < i` /\
-                        `i < 2 * k0 + 1` \/ `n0 < i` /\ `i < N0` ->
+                        `i < 2 * k0 + 1` \/ `n0 < i` /\
+                        `i < (array_length t1)` ->
                         `(access t1 i) = (access t0 i)`)) /\
                       ((v:Z) ((inftree t0 n0 v k0) -> (inftree t1 n0 v k0))) 
                       t0 result1 Post20) end) in
-                (exist_2 [t2: (array N0 Z)][result1: unit](permut t2 t0) /\
+                (exist_2 [t2: (array Z)][result1: unit](permut t2 t0) /\
                 ((i:Z) (`k0 <= i` /\ `i <= n0` -> (heap t2 n0 i))) /\
                 ((i:Z)
                  (`0 <= i` /\ `i < k0` \/ `k0 < i` /\ `i < 2 * k0 + 1` \/
-                  `n0 < i` /\ `i < N0` -> `(access t2 i) = (access t0 i)`)) /\
+                  `n0 < i` /\ `i < (array_length t2)` ->
+                  `(access t2 i) = (access t0 i)`)) /\
                 ((v:Z) ((inftree t0 n0 v k0) -> (inftree t2 n0 v k0))) 
                 t1 result0 Post18) in
-              (exist_2 [t2: (array N0 Z)][result1: unit](permut t2 t0) /\
+              (exist_2 [t2: (array Z)][result1: unit](permut t2 t0) /\
               ((i:Z) (`k0 <= i` /\ `i <= n0` -> (heap t2 n0 i))) /\
               ((i:Z)
                (`0 <= i` /\ `i < k0` \/ `k0 < i` /\ `i < 2 * k0 + 1` \/
-                `n0 < i` /\ `i < N0` -> `(access t2 i) = (access t0 i)`)) /\
+                `n0 < i` /\ `i < (array_length t2)` ->
+                `(access t2 i) = (access t0 i)`)) /\
               ((v:Z) ((inftree t0 n0 v k0) -> (inftree t2 n0 v k0))) 
               t1 result0 Post10)
           | (right Test1) =>
@@ -858,25 +846,27 @@ Definition downheap := (* validation *)
                 ((i:Z) (`k0 <= i` /\ `i <= n0` -> (heap t0 n0 i))) /\
                 ((i:Z)
                  (`0 <= i` /\ `i < k0` \/ `k0 < i` /\ `i < 2 * k0 + 1` \/
-                  `n0 < i` /\ `i < N0` -> `(access t0 i) = (access t0 i)`)) /\
+                  `n0 < i` /\ `i < (array_length t0)` ->
+                  `(access t0 i) = (access t0 i)`)) /\
                 ((v:Z) ((inftree t0 n0 v k0) -> (inftree t0 n0 v k0))) 
                 tt
-                (downheap_po_14 N k n t Pre15 Variant1 N0 k0 n0 t0 Pre14
-                Pre13 j Post2 Test1)) in
-              (exist_2 [t1: (array N0 Z)][result1: unit](permut t1 t0) /\
+                (downheap_po_14 k n t Pre15 Variant1 k0 n0 t0 Pre14 Pre13 j
+                Post2 Test1)) in
+              (exist_2 [t1: (array Z)][result1: unit](permut t1 t0) /\
               ((i:Z) (`k0 <= i` /\ `i <= n0` -> (heap t1 n0 i))) /\
               ((i:Z)
                (`0 <= i` /\ `i < k0` \/ `k0 < i` /\ `i < 2 * k0 + 1` \/
-                `n0 < i` /\ `i < N0` -> `(access t1 i) = (access t0 i)`)) /\
+                `n0 < i` /\ `i < (array_length t1)` ->
+                `(access t1 i) = (access t0 i)`)) /\
               ((v:Z) ((inftree t0 n0 v k0) -> (inftree t1 n0 v k0))) 
               t0 result0 Post9) end) in
-        (exist_2 [t2: (array N0 Z)][result0: unit](permut t2 t0) /\
+        (exist_2 [t2: (array Z)][result0: unit](permut t2 t0) /\
         ((i:Z) (`k0 <= i` /\ `i <= n0` -> (heap t2 n0 i))) /\
         ((i:Z)
          (`0 <= i` /\ `i < k0` \/ `k0 < i` /\ `i < 2 * k0 + 1` \/ `n0 < i` /\
-          `i < N0` -> `(access t2 i) = (access t0 i)`)) /\
+          `i < (array_length t2)` -> `(access t2 i) = (access t0 i)`)) /\
         ((v:Z) ((inftree t0 n0 v k0) -> (inftree t2 n0 v k0))) t1 result
-        Post7) `n - k` N k n t (refl_equal ? `n - k`) Pre15).
+        Post7) `n - k` k n t (refl_equal ? `n - k`) Pre15).
 
 
 
