examples/heapsort/heapsort_why.v
@@ -65,196 +65,225 @@ Save.
 (* Obligations. *)
 
 Lemma heapsort_po_1 : 
-  (N: Z)
-  (t: (array N Z))
-  (Pre16: `1 <= N`)
+  (t: (array Z))
+  (Pre16: `1 <= (array_length t)`)
   (result: Z)
-  (Post3: result = (Zdiv2 `N - 2`))
+  (Post3: result = (Zdiv2 `(array_length t) - 2`))
   (Variant1: Z)
   (k0: Z)
-  (t0: (array N Z))
+  (t0: (array Z))
   (Pre6: Variant1 = `k0 + 1`)
-  (Pre5: (`(-1) <= k0` /\ `k0 <= N - 1`) /\
-         ((i:Z) (`k0 + 1 <= i` /\ `i <= N - 1` -> (heap t0 `N - 1` i))) /\
+  (Pre5: (`(-1) <= k0` /\ `k0 <= (array_length t0) - 1`) /\
+         ((i:Z)
+          (`k0 + 1 <= i` /\ `i <= (array_length t0) - 1` ->
+           (heap t0 `(array_length t0) - 1` i))) /\
          (permut t0 t))
   (Test2: `k0 >= 0`)
-  (`0 <= k0` /\ `k0 <= N - 1`) /\ `N - 1 < N` /\
-  ((i:Z) (`k0 + 1 <= i` /\ `i <= N - 1` -> (heap t0 `N - 1` i))).
+  (`0 <= k0` /\ `k0 <= (array_length t0) - 1`) /\
+  `(array_length t0) - 1 < (array_length t0)` /\
+  ((i:Z)
+   (`k0 + 1 <= i` /\ `i <= (array_length t0) - 1` ->
+    (heap t0 `(array_length t0) - 1` i))).
 Proof.
 Intuition.
 Save.
 
 Lemma heapsort_po_2 : 
-  (N: Z)
-  (t: (array N Z))
-  (Pre16: `1 <= N`)
+  (t: (array Z))
+  (Pre16: `1 <= (array_length t)`)
   (result: Z)
-  (Post3: result = (Zdiv2 `N - 2`))
+  (Post3: result = (Zdiv2 `(array_length t) - 2`))
   (Variant1: Z)
   (k0: Z)
-  (t0: (array N Z))
+  (t0: (array Z))
   (Pre6: Variant1 = `k0 + 1`)
-  (Pre5: (`(-1) <= k0` /\ `k0 <= N - 1`) /\
-         ((i:Z) (`k0 + 1 <= i` /\ `i <= N - 1` -> (heap t0 `N - 1` i))) /\
+  (Pre5: (`(-1) <= k0` /\ `k0 <= (array_length t0) - 1`) /\
+         ((i:Z)
+          (`k0 + 1 <= i` /\ `i <= (array_length t0) - 1` ->
+           (heap t0 `(array_length t0) - 1` i))) /\
          (permut t0 t))
   (Test2: `k0 >= 0`)
-  (Pre4: (`0 <= k0` /\ `k0 <= N - 1`) /\ `N - 1 < N` /\
-         ((i:Z) (`k0 + 1 <= i` /\ `i <= N - 1` -> (heap t0 `N - 1` i))))
-  (t1: (array N Z))
+  (Pre4: (`0 <= k0` /\ `k0 <= (array_length t0) - 1`) /\
+         `(array_length t0) - 1 < (array_length t0)` /\
+         ((i:Z)
+          (`k0 + 1 <= i` /\ `i <= (array_length t0) - 1` ->
+           (heap t0 `(array_length t0) - 1` i))))
+  (t1: (array Z))
   (Post11: (permut t1 t0) /\
-           ((i:Z) (`k0 <= i` /\ `i <= N - 1` -> (heap t1 `N - 1` i))) /\
+           ((i:Z)
+            (`k0 <= i` /\ `i <= (array_length t0) - 1` ->
+             (heap t1 `(array_length t0) - 1` i))) /\
            ((i:Z)
             (`0 <= i` /\ `i < k0` \/ `k0 < i` /\ `i < 2 * k0 + 1` \/
-             `N - 1 < i` /\ `i < N` -> `(access t1 i) = (access t0 i)`)) /\
-           ((v:Z) ((inftree t0 `N - 1` v k0) -> (inftree t1 `N - 1` v k0))))
+             `(array_length t0) - 1 < i` /\ `i < (array_length t1)` ->
+             `(access t1 i) = (access t0 i)`)) /\
+           ((v:Z)
+            ((inftree t0 `(array_length t0) - 1` v k0) ->
+             (inftree t1 `(array_length t0) - 1` v k0))))
   (k1: Z)
   (Post1: k1 = `k0 - 1`)
-  ((`(-1) <= k1` /\ `k1 <= N - 1`) /\
-  ((i:Z) (`k1 + 1 <= i` /\ `i <= N - 1` -> (heap t1 `N - 1` i))) /\
-  (permut t1 t)) /\ (Zwf `0` `k1 + 1` `k0 + 1`).
+  ((`(-1) <= k1` /\ `k1 <= (array_length t1) - 1`) /\
+  ((i:Z)
+   (`k1 + 1 <= i` /\ `i <= (array_length t1) - 1` ->
+    (heap t1 `(array_length t1) - 1` i))) /\ (permut t1 t)) /\
+  (Zwf `0` `k1 + 1` `k0 + 1`).
 Proof.
-Intuition.
+Intuition (SameLength t1 t0; Try Omega).
+Rewrite H10; Auto with *.
 Apply permut_trans with t':=t0; Assumption.
 Unfold Zwf; Omega'.
 Save.
 
 Lemma heapsort_po_3 : 
-  (N: Z)
-  (t: (array N Z))
-  (Pre16: `1 <= N`)
+  (t: (array Z))
+  (Pre16: `1 <= (array_length t)`)
   (result: Z)
-  (Post3: result = (Zdiv2 `N - 2`))
-  (`(-1) <= result` /\ `result <= N - 1`) /\
-  ((i:Z) (`result + 1 <= i` /\ `i <= N - 1` -> (heap t `N - 1` i))) /\
-  (permut t t).
+  (Post3: result = (Zdiv2 `(array_length t) - 2`))
+  (`(-1) <= result` /\ `result <= (array_length t) - 1`) /\
+  ((i:Z)
+   (`result + 1 <= i` /\ `i <= (array_length t) - 1` ->
+    (heap t `(array_length t) - 1` i))) /\ (permut t t).
 Proof.
 Intros.
-Generalize (lem_div2_0 N Pre16); Intuition Try Omega'.
+Generalize (lem_div2_0 (array_length t) Pre16); Intuition Try Omega'.
 Apply heap_leaf.
-Generalize (lem_div2_1 N Pre16); Omega'.
-Apply (lem_div2_2 N i); Trivial Orelse Omega'.
+Generalize (lem_div2_1 (array_length t) Pre16); Omega'.
+Apply (lem_div2_2 (array_length t) i); Trivial Orelse Omega'.
 Auto with datatypes.
 Save.
 
 Lemma heapsort_po_4 : 
-  (N: Z)
-  (t: (array N Z))
-  (Pre16: `1 <= N`)
+  (t: (array Z))
+  (Pre16: `1 <= (array_length t)`)
   (result: Z)
-  (Post3: result = (Zdiv2 `N - 2`))
+  (Post3: result = (Zdiv2 `(array_length t) - 2`))
   (k0: Z)
-  (t0: (array N Z))
-  (Post2: ((`(-1) <= k0` /\ `k0 <= N - 1`) /\
-          ((i:Z) (`k0 + 1 <= i` /\ `i <= N - 1` -> (heap t0 `N - 1` i))) /\
+  (t0: (array Z))
+  (Post2: ((`(-1) <= k0` /\ `k0 <= (array_length t0) - 1`) /\
+          ((i:Z)
+           (`k0 + 1 <= i` /\ `i <= (array_length t0) - 1` ->
+            (heap t0 `(array_length t0) - 1` i))) /\
           (permut t0 t)) /\ `k0 < 0`)
-  (heap t0 `N - 1` `0`) /\ (permut t0 t).
+  (heap t0 `(array_length t0) - 1` `0`) /\ (permut t0 t).
 Proof.
 Intuition.
+SameLength t0 t; Auto with *.
 Save.
 
 Lemma heapsort_po_5 : 
-  (N: Z)
-  (t: (array N Z))
-  (Pre16: `1 <= N`)
-  (t0: (array N Z))
-  (Post9: (heap t0 `N - 1` `0`) /\ (permut t0 t))
+  (t: (array Z))
+  (Pre16: `1 <= (array_length t)`)
+  (t0: (array Z))
+  (Post9: (heap t0 `(array_length t0) - 1` `0`) /\ (permut t0 t))
   (result0: Z)
-  (Post6: result0 = `N - 1`)
+  (Post6: result0 = `(array_length t0) - 1`)
   (Variant3: Z)
   (k0: Z)
-  (t1: (array N Z))
+  (t1: (array Z))
   (Pre15: Variant3 = k0)
-  (Pre14: (`0 <= k0` /\ `k0 <= N - 1`) /\
+  (Pre14: (`0 <= k0` /\ `k0 <= (array_length t1) - 1`) /\
           ((i:Z) (`0 <= i` /\ `i <= k0` -> (heap t1 k0 i))) /\
-          ((`k0 + 1 <= N - 1` -> `(access t1 0) <= (access t1 k0 + 1)`)) /\
-          ((`k0 + 1 <= N - 1` -> (sorted_array t1 `k0 + 1` `N - 1`))) /\
+          ((`k0 + 1 <= (array_length t1) - 1` ->
+            `(access t1 0) <= (access t1 k0 + 1)`)) /\
+          ((`k0 + 1 <= (array_length t1) - 1` ->
+            (sorted_array t1 `k0 + 1` `(array_length t1) - 1`))) /\
           (permut t1 t))
   (Test4: `k0 >= 1`)
-  (`0 <= 0` /\ `0 < N`) /\ `0 <= k0` /\ `k0 < N`.
+  (`0 <= 0` /\ `0 < (array_length t1)`) /\ `0 <= k0` /\
+  `k0 < (array_length t1)`.
 Proof.
 Intuition.
 Save.
 
 Lemma heapsort_po_6 : 
-  (N: Z)
-  (t: (array N Z))
-  (Pre16: `1 <= N`)
-  (t0: (array N Z))
-  (Post9: (heap t0 `N - 1` `0`) /\ (permut t0 t))
+  (t: (array Z))
+  (Pre16: `1 <= (array_length t)`)
+  (t0: (array Z))
+  (Post9: (heap t0 `(array_length t0) - 1` `0`) /\ (permut t0 t))
   (result0: Z)
-  (Post6: result0 = `N - 1`)
+  (Post6: result0 = `(array_length t0) - 1`)
   (Variant3: Z)
   (k0: Z)
-  (t1: (array N Z))
+  (t1: (array Z))
   (Pre15: Variant3 = k0)
-  (Pre14: (`0 <= k0` /\ `k0 <= N - 1`) /\
+  (Pre14: (`0 <= k0` /\ `k0 <= (array_length t1) - 1`) /\
           ((i:Z) (`0 <= i` /\ `i <= k0` -> (heap t1 k0 i))) /\
-          ((`k0 + 1 <= N - 1` -> `(access t1 0) <= (access t1 k0 + 1)`)) /\
-          ((`k0 + 1 <= N - 1` -> (sorted_array t1 `k0 + 1` `N - 1`))) /\
+          ((`k0 + 1 <= (array_length t1) - 1` ->
+            `(access t1 0) <= (access t1 k0 + 1)`)) /\
+          ((`k0 + 1 <= (array_length t1) - 1` ->
+            (sorted_array t1 `k0 + 1` `(array_length t1) - 1`))) /\
           (permut t1 t))
   (Test4: `k0 >= 1`)
-  (Pre13: (`0 <= 0` /\ `0 < N`) /\ `0 <= k0` /\ `k0 < N`)
-  (t2: (array N Z))
+  (Pre13: (`0 <= 0` /\ `0 < (array_length t1)`) /\ `0 <= k0` /\
+          `k0 < (array_length t1)`)
+  (t2: (array Z))
   (Post15: (exchange t2 t1 `0` k0))
-  (`0 <= 0` /\ `0 <= k0 - 1`) /\ `k0 - 1 < N` /\
+  (`0 <= 0` /\ `0 <= k0 - 1`) /\ `k0 - 1 < (array_length t2)` /\
   ((i:Z) (`0 + 1 <= i` /\ `i <= k0 - 1` -> (heap t2 `k0 - 1` i))).
 Proof.
 Intuition.
+SameLength t2 t1; Omega.
 Apply heap_id with t:=t1.
 Apply heap_weakening. Omega'.
 Apply H1; Omega'. Omega'.
 Decompose [exchange] Post15; Clear Post15.
 Unfold array_id.
-Intros i0 Hi0. Symmetry. Apply H17; Omega'.
+Intros i0 Hi0. Symmetry. Apply H18; Omega'.
 Save.
 
 Lemma heapsort_po_7 : 
-  (N: Z)
-  (t: (array N Z))
-  (Pre16: `1 <= N`)
-  (t0: (array N Z))
-  (Post9: (heap t0 `N - 1` `0`) /\ (permut t0 t))
+  (t: (array Z))
+  (Pre16: `1 <= (array_length t)`)
+  (t0: (array Z))
+  (Post9: (heap t0 `(array_length t0) - 1` `0`) /\ (permut t0 t))
   (result0: Z)
-  (Post6: result0 = `N - 1`)
+  (Post6: result0 = `(array_length t0) - 1`)
   (Variant3: Z)
   (k0: Z)
-  (t1: (array N Z))
+  (t1: (array Z))
   (Pre15: Variant3 = k0)
-  (Pre14: (`0 <= k0` /\ `k0 <= N - 1`) /\
+  (Pre14: (`0 <= k0` /\ `k0 <= (array_length t1) - 1`) /\
           ((i:Z) (`0 <= i` /\ `i <= k0` -> (heap t1 k0 i))) /\
-          ((`k0 + 1 <= N - 1` -> `(access t1 0) <= (access t1 k0 + 1)`)) /\
-          ((`k0 + 1 <= N - 1` -> (sorted_array t1 `k0 + 1` `N - 1`))) /\
+          ((`k0 + 1 <= (array_length t1) - 1` ->
+            `(access t1 0) <= (access t1 k0 + 1)`)) /\
+          ((`k0 + 1 <= (array_length t1) - 1` ->
+            (sorted_array t1 `k0 + 1` `(array_length t1) - 1`))) /\
           (permut t1 t))
   (Test4: `k0 >= 1`)
-  (Pre13: (`0 <= 0` /\ `0 < N`) /\ `0 <= k0` /\ `k0 < N`)
-  (t2: (array N Z))
+  (Pre13: (`0 <= 0` /\ `0 < (array_length t1)`) /\ `0 <= k0` /\
+          `k0 < (array_length t1)`)
+  (t2: (array Z))
   (Post15: (exchange t2 t1 `0` k0))
-  (Pre12: (`0 <= 0` /\ `0 <= k0 - 1`) /\ `k0 - 1 < N` /\
+  (Pre12: (`0 <= 0` /\ `0 <= k0 - 1`) /\ `k0 - 1 < (array_length t2)` /\
           ((i:Z) (`0 + 1 <= i` /\ `i <= k0 - 1` -> (heap t2 `k0 - 1` i))))
-  (t3: (array N Z))
+  (t3: (array Z))
   (Post17: (permut t3 t2) /\
            ((i:Z) (`0 <= i` /\ `i <= k0 - 1` -> (heap t3 `k0 - 1` i))) /\
            ((i:Z)
             (`0 <= i` /\ `i < 0` \/ `0 < i` /\ `i < 2 * 0 + 1` \/
-             `k0 - 1 < i` /\ `i < N` -> `(access t3 i) = (access t2 i)`)) /\
+             `k0 - 1 < i` /\ `i < (array_length t3)` ->
+             `(access t3 i) = (access t2 i)`)) /\
            ((v:Z)
             ((inftree t2 `k0 - 1` v `0`) -> (inftree t3 `k0 - 1` v `0`))))
   (k1: Z)
   (Post4: k1 = `k0 - 1`)
-  ((`0 <= k1` /\ `k1 <= N - 1`) /\
+  ((`0 <= k1` /\ `k1 <= (array_length t3) - 1`) /\
   ((i:Z) (`0 <= i` /\ `i <= k1` -> (heap t3 k1 i))) /\
-  ((`k1 + 1 <= N - 1` -> `(access t3 0) <= (access t3 k1 + 1)`)) /\
-  ((`k1 + 1 <= N - 1` -> (sorted_array t3 `k1 + 1` `N - 1`))) /\
-  (permut t3 t)) /\ (Zwf `0` k1 k0).
+  ((`k1 + 1 <= (array_length t3) - 1` ->
+    `(access t3 0) <= (access t3 k1 + 1)`)) /\
+  ((`k1 + 1 <= (array_length t3) - 1` ->
+    (sorted_array t3 `k1 + 1` `(array_length t3) - 1`))) /\ (permut t3 t)) /\
+  (Zwf `0` k1 k0).
 Proof.
 Intuition.
+SameLength t3 t2; Omega.
 (* heap *)
 Subst k1; Apply H17; Omega'.
 (* t[0] <= t[k] *)
 Subst k1; Ring `k0-1+1`. 
 Rewrite (H16 k0); [ Idtac | Omega' ].
 Decompose [exchange] Post15.
-Rewrite H23.
+Rewrite H24.
 Apply inftree_1 with n:=`k0-1`.
 Apply H19.
 Apply inftree_weakening. Omega'.
@@ -264,27 +293,32 @@ Apply H1; Omega'.
 Assumption. Omega'.
 (* sorted *)
 Subst k1; Ring `k0-1+1`.  
-Elim (Z_le_lt_eq_dec k0 `N-1` H6); Intro.
+Elim (Z_le_lt_eq_dec k0 `(array_length t1)-1` H6); Intro.
   (* k0 < N-1 *)
   Replace k0 with `(k0+1)-1`; [ Idtac | Omega' ].
   Apply left_extension. Omega'. Omega'.
   Apply sorted_array_id with t1:=t2. 
   Apply sorted_array_id with t1:=t1. 
-  Apply H7; Omega'.
+  SameLength t3 t2; SameLength t2 t1; SameLength t1 t.
+  Rewrite H20; Rewrite H21. Apply H7; Omega'.
   Decompose [exchange] Post15.
-  Unfold array_id. Intros i Hi. Symmetry. Apply H24; Omega'.
+  Unfold array_id. Intros i Hi. Symmetry. 
+  SameLength t3 t2; Apply H25; Try Omega'.
   Unfold array_id. Intros i Hi. Symmetry. Apply H16; Omega'.
   (* t3[k0] <= t3[k0+1] *)
   Ring `k0+1-1`. 
   Rewrite (H16 k0); [ Idtac | Omega' ].
-  Rewrite (H16 `k0+1`); [ Idtac | Omega' ].
+  Rewrite (H16 `k0+1`); 
+    [ Idtac | SameLength t3 t2; SameLength t2 t1; Omega' ].
   Decompose [exchange] Post15.
-  Rewrite H23. Rewrite (H24 `k0+1`); [ Idtac | Omega' | Omega' | Omega' ].
+  Rewrite H24. Rewrite (H25 `k0+1`); [ Idtac | Omega' | Omega' | Omega' ].
   Apply H4; Omega'.
   (* k0 = N-1 *)
   Rewrite b. 
   Unfold sorted_array.
-  Intros HN x HHx Hx. Absurd `x >= N-1`; Omega'.
+  Intros HN x HHx Hx. 
+  Absurd `x >= (array_length t3)-1`; 
+  SameLength t3 t2; SameLength t2 t1; Omega'.
 (* (permut t3 t) *)
 Apply permut_trans with t':=t2; Try Assumption. 
 Apply permut_trans with t':=t1.
@@ -295,90 +329,103 @@ Unfold Zwf; Omega'.
 Save.
 
 Lemma heapsort_po_8 : 
-  (N: Z)
-  (t: (array N Z))
-  (Pre16: `1 <= N`)
-  (t0: (array N Z))
-  (Post9: (heap t0 `N - 1` `0`) /\ (permut t0 t))
+  (t: (array Z))
+  (Pre16: `1 <= (array_length t)`)
+  (t0: (array Z))
+  (Post9: (heap t0 `(array_length t0) - 1` `0`) /\ (permut t0 t))
   (result0: Z)
-  (Post6: result0 = `N - 1`)
-  (`0 <= result0` /\ `result0 <= N - 1`) /\
+  (Post6: result0 = `(array_length t0) - 1`)
+  (`0 <= result0` /\ `result0 <= (array_length t0) - 1`) /\
   ((i:Z) (`0 <= i` /\ `i <= result0` -> (heap t0 result0 i))) /\
-  ((`result0 + 1 <= N - 1` -> `(access t0 0) <= (access t0 result0 + 1)`)) /\
-  ((`result0 + 1 <= N - 1` -> (sorted_array t0 `result0 + 1` `N - 1`))) /\
+  ((`result0 + 1 <= (array_length t0) - 1` ->
+    `(access t0 0) <= (access t0 result0 + 1)`)) /\
+  ((`result0 + 1 <= (array_length t0) - 1` ->
+    (sorted_array t0 `result0 + 1` `(array_length t0) - 1`))) /\
   (permut t0 t).
 Proof.
-Intuition.
+Intuition SameLength t0 t; Try Omega.
 Apply heap_all.
 Subst result0; Assumption.
 Tauto.
-Intro; Absurd `N-1+1 <= N-1`; Omega'.
+Intro; Absurd `(array_length t0)-1+1 <= (array_length t0)-1`; Omega'.
 Save.
 
 Lemma heapsort_po_9 : 
-  (N: Z)
-  (t: (array N Z))
-  (Pre16: `1 <= N`)
-  (t0: (array N Z))
-  (Post9: (heap t0 `N - 1` `0`) /\ (permut t0 t))
+  (t: (array Z))
+  (Pre16: `1 <= (array_length t)`)
+  (t0: (array Z))
+  (Post9: (heap t0 `(array_length t0) - 1` `0`) /\ (permut t0 t))
   (result0: Z)
-  (Post6: result0 = `N - 1`)
+  (Post6: result0 = `(array_length t0) - 1`)
   (k0: Z)
-  (t1: (array N Z))
-  (Post5: ((`0 <= k0` /\ `k0 <= N - 1`) /\
+  (t1: (array Z))
+  (Post5: ((`0 <= k0` /\ `k0 <= (array_length t1) - 1`) /\
           ((i:Z) (`0 <= i` /\ `i <= k0` -> (heap t1 k0 i))) /\
-          ((`k0 + 1 <= N - 1` -> `(access t1 0) <= (access t1 k0 + 1)`)) /\
-          ((`k0 + 1 <= N - 1` -> (sorted_array t1 `k0 + 1` `N - 1`))) /\
+          ((`k0 + 1 <= (array_length t1) - 1` ->
+            `(access t1 0) <= (access t1 k0 + 1)`)) /\
+          ((`k0 + 1 <= (array_length t1) - 1` ->
+            (sorted_array t1 `k0 + 1` `(array_length t1) - 1`))) /\
           (permut t1 t)) /\ `k0 < 1`)
-  (sorted_array t1 `0` `N - 1`) /\ (permut t1 t).
+  (sorted_array t1 `0` `(array_length t1) - 1`) /\ (permut t1 t).
 Proof.
 Intuition.
-Elim (Z_le_lt_eq_dec `1` N Pre16); Intro.
+Elim (Z_le_lt_eq_dec `1` (array_length t) Pre16); Intro.
   (* 1 < N *)
   Replace `0` with `1-1`; [ Idtac | Omega' ].
   Apply left_extension. Omega'. Omega'.
   Replace `1` with `k0+1`; [ Idtac | Omega' ].
-  Replace `N-(k0+1)` with `N-1`; [ Idtac | Omega' ].
-  Apply H6; Omega'.
+  Replace `(array_length t1)-(k0+1)` with `(array_length t1)-1`; 
+  [ Idtac | Omega' ].
+  Apply H6; SameLength t1 t; Omega'.
   Replace `1-1` with `0`; [ Idtac | Omega' ]. (* Ring `1-1`. *)
   Replace `1` with `k0+1`; [ Idtac | Omega' ].
-  Apply H4; Omega'.
+  Apply H4; SameLength t1 t; Omega'.
   (* 1 = N *)
   Unfold sorted_array. 
-  Intros HN x HHx Hx. Absurd `x >= N-1`; Omega'.
+  Intros HN x HHx Hx. 
+  Absurd `x >= (array_length t)-1`; SameLength t1 t; Omega'.
 Save.
 
 Require swap_why.
 Require downheap_why.
 
 Definition heapsort := (* validation *)
-  [N: Z; t: (array N Z); Pre16: `1 <= N`]
+  [t: (array Z); Pre16: `1 <= (array_length t)`]
     let (t0, result, Post9) =
       let (result, Post3) = (exist_1 [result: Z]
-        result = (Zdiv2 `N - 2`) (Zdiv2 `N - 2`)
-        (refl_equal ? (Zdiv2 `N - 2`))) in
+        result = (Zdiv2 `(array_length t) - 2`) (Zdiv2 `(array_length t) - 2`)
+        (refl_equal ? (Zdiv2 `(array_length t) - 2`))) in
       let (k0, t0, result0, Post2) =
         (well_founded_induction Z (Zwf ZERO) (Zwf_well_founded `0`)
-          [Variant1: Z](k0: Z)(t0: (array N Z))(_: Variant1 = `k0 + 1`)
-          (_0: (`(-1) <= k0` /\ `k0 <= N - 1`) /\
-          ((i:Z) (`k0 + 1 <= i` /\ `i <= N - 1` -> (heap t0 `N - 1` i))) /\
-          (permut t0 t))
-          (sig_3 Z (array N Z) unit [k1: Z][t1: (array N Z)][result0: unit]
-           (((`(-1) <= k1` /\ `k1 <= N - 1`) /\
-           ((i:Z) (`k1 + 1 <= i` /\ `i <= N - 1` -> (heap t1 `N - 1` i))) /\
+          [Variant1: Z](k0: Z)(t0: (array Z))(_: Variant1 = `k0 + 1`)
+          (_0: (`(-1) <= k0` /\ `k0 <= (array_length t0) - 1`) /\
+          ((i:Z)
+           (`k0 + 1 <= i` /\ `i <= (array_length t0) - 1` ->
+            (heap t0 `(array_length t0) - 1` i))) /\ (permut t0 t))
+          (sig_3 Z (array Z) unit [k1: Z][t1: (array Z)][result0: unit]
+           (((`(-1) <= k1` /\ `k1 <= (array_length t1) - 1`) /\
+           ((i:Z)
+            (`k1 + 1 <= i` /\ `i <= (array_length t1) - 1` ->
+             (heap t1 `(array_length t1) - 1` i))) /\
            (permut t1 t)) /\ `k1 < 0`))
           [Variant1: Z; wf1: (Variant2: Z)(Pre1: (Zwf `0` Variant2 Variant1))
-           (k0: Z)(t0: (array N Z))(_: Variant2 = `k0 + 1`)
-           (_0: (`(-1) <= k0` /\ `k0 <= N - 1`) /\
-           ((i:Z) (`k0 + 1 <= i` /\ `i <= N - 1` -> (heap t0 `N - 1` i))) /\
+           (k0: Z)(t0: (array Z))(_: Variant2 = `k0 + 1`)
+           (_0: (`(-1) <= k0` /\ `k0 <= (array_length t0) - 1`) /\
+           ((i:Z)
+            (`k0 + 1 <= i` /\ `i <= (array_length t0) - 1` ->
+             (heap t0 `(array_length t0) - 1` i))) /\
            (permut t0 t))
-           (sig_3 Z (array N Z) unit [k1: Z][t1: (array N Z)][result0: unit]
-            (((`(-1) <= k1` /\ `k1 <= N - 1`) /\
-            ((i:Z) (`k1 + 1 <= i` /\ `i <= N - 1` -> (heap t1 `N - 1` i))) /\
+           (sig_3 Z (array Z) unit [k1: Z][t1: (array Z)][result0: unit]
+            (((`(-1) <= k1` /\ `k1 <= (array_length t1) - 1`) /\
+            ((i:Z)
+             (`k1 + 1 <= i` /\ `i <= (array_length t1) - 1` ->
+              (heap t1 `(array_length t1) - 1` i))) /\
             (permut t1 t)) /\ `k1 < 0`));
-           k0: Z; t0: (array N Z); Pre6: Variant1 = `k0 + 1`;
-           Pre5: (`(-1) <= k0` /\ `k0 <= N - 1`) /\
-           ((i:Z) (`k0 + 1 <= i` /\ `i <= N - 1` -> (heap t0 `N - 1` i))) /\
+           k0: Z; t0: (array Z); Pre6: Variant1 = `k0 + 1`;
+           Pre5: (`(-1) <= k0` /\ `k0 <= (array_length t0) - 1`) /\
+           ((i:Z)
+            (`k0 + 1 <= i` /\ `i <= (array_length t0) - 1` ->
+             (heap t0 `(array_length t0) - 1` i))) /\
            (permut t0 t)]
             let (result0, Bool1) =
               let (result2, Post10) = (Z_ge_lt_bool k0 `0`) in
@@ -391,24 +438,26 @@ Definition heapsort := (* validation *)
                 let (k1, t1, result1, Post2) =
                   let (k1, t1, result1, Post8) =
                     let Pre4 =
-                      (heapsort_po_1 N t Pre16 result Post3 Variant1 k0 t0
-                      Pre6 Pre5 Test2) in
+                      (heapsort_po_1 t Pre16 result Post3 Variant1 k0 t0 Pre6
+                      Pre5 Test2) in
                     let (t1, result1, Post11) =
                       let Pre2 = Pre4 in
                       let Pre3 = Pre2 in
                       let (t1, result3, Post12) =
-                        (downheap N k0 `N - 1` t0 Pre2) in
-                      (exist_2 [t2: (array N Z)][result4: unit]
+                        (downheap k0 `(array_length t0) - 1` t0 Pre2) in
+                      (exist_2 [t2: (array Z)][result4: unit]
                       (permut t2 t0) /\
                       ((i:Z)
-                       (`k0 <= i` /\ `i <= N - 1` -> (heap t2 `N - 1` i))) /\
+                       (`k0 <= i` /\ `i <= (array_length t0) - 1` ->
+                        (heap t2 `(array_length t0) - 1` i))) /\
                       ((i:Z)
                        (`0 <= i` /\ `i < k0` \/ `k0 < i` /\
-                        `i < 2 * k0 + 1` \/ `N - 1 < i` /\ `i < N` ->
+                        `i < 2 * k0 + 1` \/ `(array_length t0) - 1 < i` /\
+                        `i < (array_length t2)` ->
                         `(access t2 i) = (access t0 i)`)) /\
                       ((v:Z)
-                       ((inftree t0 `N - 1` v k0) ->
-                        (inftree t2 `N - 1` v k0))) t1
+                       ((inftree t0 `(array_length t0) - 1` v k0) ->
+                        (inftree t2 `(array_length t0) - 1` v k0))) t1
                       result3 Post12) in
                     let (k1, result2, Post1) =
                       let (result2, Post1) = (exist_1 [result2: Z]
@@ -416,72 +465,89 @@ Definition heapsort := (* validation *)
                         (refl_equal ? `k0 - 1`)) in
                       (exist_2 [k2: Z][result3: unit]k2 = `k0 - 1` result2 
                       tt Post1) in
-                    (exist_3 [k2: Z][t2: (array N Z)][result3: unit]
-                    ((`(-1) <= k2` /\ `k2 <= N - 1`) /\
+                    (exist_3 [k2: Z][t2: (array Z)][result3: unit]
+                    ((`(-1) <= k2` /\ `k2 <= (array_length t2) - 1`) /\
                     ((i:Z)
-                     (`k2 + 1 <= i` /\ `i <= N - 1` -> (heap t2 `N - 1` i))) /\
+                     (`k2 + 1 <= i` /\ `i <= (array_length t2) - 1` ->
+                      (heap t2 `(array_length t2) - 1` i))) /\
                     (permut t2 t)) /\ (Zwf `0` `k2 + 1` `k0 + 1`) k1 
                     t1 result2
-                    (heapsort_po_2 N t Pre16 result Post3 Variant1 k0 t0 Pre6
+                    (heapsort_po_2 t Pre16 result Post3 Variant1 k0 t0 Pre6
                     Pre5 Test2 Pre4 t1 Post11 k1 Post1)) in
                   ((wf1 `k1 + 1`) (loop_variant_1 Pre6 Post8) k1 t1
                     (refl_equal ? `k1 + 1`) (proj1 ? ? Post8)) in
-                (exist_3 [k2: Z][t2: (array N Z)][result2: unit]
-                ((`(-1) <= k2` /\ `k2 <= N - 1`) /\
-                ((i:Z) (`k2 + 1 <= i` /\ `i <= N - 1` -> (heap t2 `N - 1` i))) /\
+                (exist_3 [k2: Z][t2: (array Z)][result2: unit]
+                ((`(-1) <= k2` /\ `k2 <= (array_length t2) - 1`) /\
+                ((i:Z)
+                 (`k2 + 1 <= i` /\ `i <= (array_length t2) - 1` ->
+                  (heap t2 `(array_length t2) - 1` i))) /\
                 (permut t2 t)) /\ `k2 < 0` k1 t1 result1 Post2)
             | (right Test1) =>
                 let (k1, t1, result1, Post2) = (exist_3 [k1: Z]
-                  [t1: (array N Z)][result1: unit]((`(-1) <= k1` /\
-                  `k1 <= N - 1`) /\
+                  [t1: (array Z)][result1: unit]((`(-1) <= k1` /\
+                  `k1 <= (array_length t1) - 1`) /\
                   ((i:Z)
-                   (`k1 + 1 <= i` /\ `i <= N - 1` -> (heap t1 `N - 1` i))) /\
+                   (`k1 + 1 <= i` /\ `i <= (array_length t1) - 1` ->
+                    (heap t1 `(array_length t1) - 1` i))) /\
                   (permut t1 t)) /\ `k1 < 0` k0 t0 tt
                   (conj ? ? Pre5 Test1)) in
-                (exist_3 [k2: Z][t2: (array N Z)][result2: unit]
-                ((`(-1) <= k2` /\ `k2 <= N - 1`) /\
-                ((i:Z) (`k2 + 1 <= i` /\ `i <= N - 1` -> (heap t2 `N - 1` i))) /\
+                (exist_3 [k2: Z][t2: (array Z)][result2: unit]
+                ((`(-1) <= k2` /\ `k2 <= (array_length t2) - 1`) /\
+                ((i:Z)
+                 (`k2 + 1 <= i` /\ `i <= (array_length t2) - 1` ->
+                  (heap t2 `(array_length t2) - 1` i))) /\
                 (permut t2 t)) /\ `k2 < 0` k1 t1 result1 Post2) end)
           `result + 1` result t (refl_equal ? `result + 1`)
-          (heapsort_po_3 N t Pre16 result Post3)) in
-      (exist_2 [t1: (array N Z)][result1: unit](heap t1 `N - 1` `0`) /\
-      (permut t1 t) t0 result0
-      (heapsort_po_4 N t Pre16 result Post3 k0 t0 Post2)) in
+          (heapsort_po_3 t Pre16 result Post3)) in
+      (exist_2 [t1: (array Z)][result1: unit]
+      (heap t1 `(array_length t1) - 1` `0`) /\ (permut t1 t) t0 result0
+      (heapsort_po_4 t Pre16 result Post3 k0 t0 Post2)) in
     let (t1, result0, Post13) =
-      let (result0, Post6) = (exist_1 [result0: Z]result0 = `N - 1` `N - 1`
-        (refl_equal ? `N - 1`)) in
+      let (result0, Post6) = (exist_1 [result0: Z]
+        result0 = `(array_length t0) - 1` `(array_length t0) - 1`
+        (refl_equal ? `(array_length t0) - 1`)) in
       let (k0, t1, result1, Post5) =
         (well_founded_induction Z (Zwf ZERO) (Zwf_well_founded `0`)
-          [Variant3: Z](k0: Z)(t1: (array N Z))(_: Variant3 = k0)
-          (_0: (`0 <= k0` /\ `k0 <= N - 1`) /\
+          [Variant3: Z](k0: Z)(t1: (array Z))(_: Variant3 = k0)
+          (_0: (`0 <= k0` /\ `k0 <= (array_length t1) - 1`) /\
           ((i:Z) (`0 <= i` /\ `i <= k0` -> (heap t1 k0 i))) /\
-          ((`k0 + 1 <= N - 1` -> `(access t1 0) <= (access t1 k0 + 1)`)) /\
-          ((`k0 + 1 <= N - 1` -> (sorted_array t1 `k0 + 1` `N - 1`))) /\
+          ((`k0 + 1 <= (array_length t1) - 1` ->
+            `(access t1 0) <= (access t1 k0 + 1)`)) /\
+          ((`k0 + 1 <= (array_length t1) - 1` ->
+            (sorted_array t1 `k0 + 1` `(array_length t1) - 1`))) /\
           (permut t1 t))
-          (sig_3 Z (array N Z) unit [k1: Z][t2: (array N Z)][result1: unit]
-           (((`0 <= k1` /\ `k1 <= N - 1`) /\
+          (sig_3 Z (array Z) unit [k1: Z][t2: (array Z)][result1: unit]
+           (((`0 <= k1` /\ `k1 <= (array_length t2) - 1`) /\
            ((i:Z) (`0 <= i` /\ `i <= k1` -> (heap t2 k1 i))) /\
-           ((`k1 + 1 <= N - 1` -> `(access t2 0) <= (access t2 k1 + 1)`)) /\
-           ((`k1 + 1 <= N - 1` -> (sorted_array t2 `k1 + 1` `N - 1`))) /\
+           ((`k1 + 1 <= (array_length t2) - 1` ->
+             `(access t2 0) <= (access t2 k1 + 1)`)) /\
+           ((`k1 + 1 <= (array_length t2) - 1` ->
+             (sorted_array t2 `k1 + 1` `(array_length t2) - 1`))) /\
            (permut t2 t)) /\ `k1 < 1`))
           [Variant3: Z; wf2: (Variant4: Z)(Pre7: (Zwf `0` Variant4 Variant3))
-           (k0: Z)(t1: (array N Z))(_: Variant4 = k0)(_0: (`0 <= k0` /\
-           `k0 <= N - 1`) /\
+           (k0: Z)(t1: (array Z))(_: Variant4 = k0)(_0: (`0 <= k0` /\
+           `k0 <= (array_length t1) - 1`) /\
            ((i:Z) (`0 <= i` /\ `i <= k0` -> (heap t1 k0 i))) /\
-           ((`k0 + 1 <= N - 1` -> `(access t1 0) <= (access t1 k0 + 1)`)) /\
-           ((`k0 + 1 <= N - 1` -> (sorted_array t1 `k0 + 1` `N - 1`))) /\
+           ((`k0 + 1 <= (array_length t1) - 1` ->
+             `(access t1 0) <= (access t1 k0 + 1)`)) /\
+           ((`k0 + 1 <= (array_length t1) - 1` ->
+             (sorted_array t1 `k0 + 1` `(array_length t1) - 1`))) /\
            (permut t1 t))
-           (sig_3 Z (array N Z) unit [k1: Z][t2: (array N Z)][result1: unit]
-            (((`0 <= k1` /\ `k1 <= N - 1`) /\
+           (sig_3 Z (array Z) unit [k1: Z][t2: (array Z)][result1: unit]
+            (((`0 <= k1` /\ `k1 <= (array_length t2) - 1`) /\
             ((i:Z) (`0 <= i` /\ `i <= k1` -> (heap t2 k1 i))) /\
-            ((`k1 + 1 <= N - 1` -> `(access t2 0) <= (access t2 k1 + 1)`)) /\
-            ((`k1 + 1 <= N - 1` -> (sorted_array t2 `k1 + 1` `N - 1`))) /\
+            ((`k1 + 1 <= (array_length t2) - 1` ->
+              `(access t2 0) <= (access t2 k1 + 1)`)) /\
+            ((`k1 + 1 <= (array_length t2) - 1` ->
+              (sorted_array t2 `k1 + 1` `(array_length t2) - 1`))) /\
             (permut t2 t)) /\ `k1 < 1`));
-           k0: Z; t1: (array N Z); Pre15: Variant3 = k0; Pre14: (`0 <= k0` /\
-           `k0 <= N - 1`) /\
+           k0: Z; t1: (array Z); Pre15: Variant3 = k0; Pre14: (`0 <= k0` /\
+           `k0 <= (array_length t1) - 1`) /\
            ((i:Z) (`0 <= i` /\ `i <= k0` -> (heap t1 k0 i))) /\
-           ((`k0 + 1 <= N - 1` -> `(access t1 0) <= (access t1 k0 + 1)`)) /\
-           ((`k0 + 1 <= N - 1` -> (sorted_array t1 `k0 + 1` `N - 1`))) /\
+           ((`k0 + 1 <= (array_length t1) - 1` ->
+             `(access t1 0) <= (access t1 k0 + 1)`)) /\
+           ((`k0 + 1 <= (array_length t1) - 1` ->
+             (sorted_array t1 `k0 + 1` `(array_length t1) - 1`))) /\
            (permut t1 t)]
             let (result1, Bool2) =
               let (result3, Post14) = (Z_ge_lt_bool k0 `1`) in
@@ -494,29 +560,29 @@ Definition heapsort := (* validation *)
                 let (k1, t2, result2, Post5) =
                   let (k1, t2, result2, Post7) =
                     let Pre13 =
-                      (heapsort_po_5 N t Pre16 t0 Post9 result0 Post6
-                      Variant3 k0 t1 Pre15 Pre14 Test4) in
+                      (heapsort_po_5 t Pre16 t0 Post9 result0 Post6 Variant3
+                      k0 t1 Pre15 Pre14 Test4) in
                     let (t2, result2, Post15) =
                       let Pre8 = Pre13 in
                       let Pre9 = Pre8 in
-                      let (t2, result4, Post16) = (swap N `0` k0 t1 Pre8) in
-                      (exist_2 [t3: (array N Z)][result5: unit]
+                      let (t2, result4, Post16) = (swap `0` k0 t1 Pre8) in
+                      (exist_2 [t3: (array Z)][result5: unit]
                       (exchange t3 t1 `0` k0) t2 result4 Post16) in
                     let Pre12 =
-                      (heapsort_po_6 N t Pre16 t0 Post9 result0 Post6
-                      Variant3 k0 t1 Pre15 Pre14 Test4 Pre13 t2 Post15) in
+                      (heapsort_po_6 t Pre16 t0 Post9 result0 Post6 Variant3
+                      k0 t1 Pre15 Pre14 Test4 Pre13 t2 Post15) in
                     let (t3, result3, Post17) =
                       let Pre10 = Pre12 in
                       let Pre11 = Pre10 in
                       let (t3, result5, Post18) =
-                        (downheap N `0` `k0 - 1` t2 Pre10) in
-                      (exist_2 [t4: (array N Z)][result6: unit]
+                        (downheap `0` `k0 - 1` t2 Pre10) in
+                      (exist_2 [t4: (array Z)][result6: unit]
                       (permut t4 t2) /\
                       ((i:Z)
                        (`0 <= i` /\ `i <= k0 - 1` -> (heap t4 `k0 - 1` i))) /\
                       ((i:Z)
                        (`0 <= i` /\ `i < 0` \/ `0 < i` /\ `i < 2 * 0 + 1` \/
-                        `k0 - 1 < i` /\ `i < N` ->
+                        `k0 - 1 < i` /\ `i < (array_length t4)` ->
                         `(access t4 i) = (access t2 i)`)) /\
                       ((v:Z)
                        ((inftree t2 `k0 - 1` v `0`) ->
@@ -528,45 +594,52 @@ Definition heapsort := (* validation *)
                         (refl_equal ? `k0 - 1`)) in
                       (exist_2 [k2: Z][result5: unit]k2 = `k0 - 1` result4 
                       tt Post4) in
-                    (exist_3 [k2: Z][t4: (array N Z)][result5: unit]
-                    ((`0 <= k2` /\ `k2 <= N - 1`) /\
+                    (exist_3 [k2: Z][t4: (array Z)][result5: unit]
+                    ((`0 <= k2` /\ `k2 <= (array_length t4) - 1`) /\
                     ((i:Z) (`0 <= i` /\ `i <= k2` -> (heap t4 k2 i))) /\
-                    ((`k2 + 1 <= N - 1` ->
+                    ((`k2 + 1 <= (array_length t4) - 1` ->
                       `(access t4 0) <= (access t4 k2 + 1)`)) /\
-                    ((`k2 + 1 <= N - 1` -> (sorted_array t4 `k2 + 1` `N - 1`))) /\
+                    ((`k2 + 1 <= (array_length t4) - 1` ->
+                      (sorted_array t4 `k2 + 1` `(array_length t4) - 1`))) /\
                     (permut t4 t)) /\ (Zwf `0` k2 k0) k1 t3 result4
-                    (heapsort_po_7 N t Pre16 t0 Post9 result0 Post6 Variant3
-                    k0 t1 Pre15 Pre14 Test4 Pre13 t2 Post15 Pre12 t3 Post17
-                    k1 Post4)) in
+                    (heapsort_po_7 t Pre16 t0 Post9 result0 Post6 Variant3 k0
+                    t1 Pre15 Pre14 Test4 Pre13 t2 Post15 Pre12 t3 Post17 k1
+                    Post4)) in
                   ((wf2 k1) (loop_variant_1 Pre15 Post7) k1 t2
                     (refl_equal ? k1) (proj1 ? ? Post7)) in
-                (exist_3 [k2: Z][t3: (array N Z)][result3: unit]
-                ((`0 <= k2` /\ `k2 <= N - 1`) /\
+                (exist_3 [k2: Z][t3: (array Z)][result3: unit]((`0 <= k2` /\
+                `k2 <= (array_length t3) - 1`) /\
                 ((i:Z) (`0 <= i` /\ `i <= k2` -> (heap t3 k2 i))) /\
-                ((`k2 + 1 <= N - 1` -> `(access t3 0) <= (access t3 k2 + 1)`)) /\
-                ((`k2 + 1 <= N - 1` -> (sorted_array t3 `k2 + 1` `N - 1`))) /\
+                ((`k2 + 1 <= (array_length t3) - 1` ->
+                  `(access t3 0) <= (access t3 k2 + 1)`)) /\
+                ((`k2 + 1 <= (array_length t3) - 1` ->
+                  (sorted_array t3 `k2 + 1` `(array_length t3) - 1`))) /\
                 (permut t3 t)) /\ `k2 < 1` k1 t2 result2 Post5)
             | (right Test3) =>
                 let (k1, t2, result2, Post5) = (exist_3 [k1: Z]
-                  [t2: (array N Z)][result2: unit]((`0 <= k1` /\
-                  `k1 <= N - 1`) /\
+                  [t2: (array Z)][result2: unit]((`0 <= k1` /\
+                  `k1 <= (array_length t2) - 1`) /\
                   ((i:Z) (`0 <= i` /\ `i <= k1` -> (heap t2 k1 i))) /\
-                  ((`k1 + 1 <= N - 1` ->
+                  ((`k1 + 1 <= (array_length t2) - 1` ->
                     `(access t2 0) <= (access t2 k1 + 1)`)) /\
-                  ((`k1 + 1 <= N - 1` -> (sorted_array t2 `k1 + 1` `N - 1`))) /\
+                  ((`k1 + 1 <= (array_length t2) - 1` ->
+                    (sorted_array t2 `k1 + 1` `(array_length t2) - 1`))) /\
                   (permut t2 t)) /\ `k1 < 1` k0 t1 tt
                   (conj ? ? Pre14 Test3)) in
-                (exist_3 [k2: Z][t3: (array N Z)][result3: unit]
-                ((`0 <= k2` /\ `k2 <= N - 1`) /\
+                (exist_3 [k2: Z][t3: (array Z)][result3: unit]((`0 <= k2` /\
+                `k2 <= (array_length t3) - 1`) /\
                 ((i:Z) (`0 <= i` /\ `i <= k2` -> (heap t3 k2 i))) /\
-                ((`k2 + 1 <= N - 1` -> `(access t3 0) <= (access t3 k2 + 1)`)) /\
-                ((`k2 + 1 <= N - 1` -> (sorted_array t3 `k2 + 1` `N - 1`))) /\
+                ((`k2 + 1 <= (array_length t3) - 1` ->
+                  `(access t3 0) <= (access t3 k2 + 1)`)) /\
+                ((`k2 + 1 <= (array_length t3) - 1` ->
+                  (sorted_array t3 `k2 + 1` `(array_length t3) - 1`))) /\
                 (permut t3 t)) /\ `k2 < 1` k1 t2 result2 Post5) end) 
           result0 result0 t0 (refl_equal ? result0)
-          (heapsort_po_8 N t Pre16 t0 Post9 result0 Post6)) in
-      (exist_2 [t2: (array N Z)][result2: unit]
-      (sorted_array t2 `0` `N - 1`) /\ (permut t2 t) t1 result1
-      (heapsort_po_9 N t Pre16 t0 Post9 result0 Post6 k0 t1 Post5)) in
-    (exist_2 [t2: (array N Z)][result1: unit](sorted_array t2 `0` `N - 1`) /\
-    (permut t2 t) t1 result0 Post13).
+          (heapsort_po_8 t Pre16 t0 Post9 result0 Post6)) in
+      (exist_2 [t2: (array Z)][result2: unit]
+      (sorted_array t2 `0` `(array_length t2) - 1`) /\ (permut t2 t) 
+      t1 result1 (heapsort_po_9 t Pre16 t0 Post9 result0 Post6 k0 t1 Post5)) in
+    (exist_2 [t2: (array Z)][result1: unit]
+    (sorted_array t2 `0` `(array_length t2) - 1`) /\ (permut t2 t) t1 
+    result0 Post13).
 
